src/coq/Handlers/FiniteMemoryTheory.v
@@ -1,0 +1,3153 @@
+(* begin hide *)
+From Coq Require Import
+     Morphisms ZArith List String Lia
+     FSets.FMapAVL
+     Structures.OrderedTypeEx
+     micromega.Lia
+     Psatz.
+
+From ITree Require Import
+     ITree
+     Basics.Basics
+     Events.Exception
+     Eq.Eq
+     Events.StateFacts
+     Events.State.
+
+Import Basics.Basics.Monads.
+
+From ExtLib Require Import
+     Structures.Monads
+     Structures.Functor
+     Programming.Eqv
+     Data.String.
+
+From Vellvm Require Import
+     Numeric.Coqlib
+     Numeric.Integers
+     Numeric.Floats
+     Utils.Tactics
+     Utils.Util
+     Utils.Error
+     Utils.IntMaps
+     Utils.ListUtil
+     Syntax.LLVMAst
+     Syntax.DynamicTypes
+     Syntax.DataLayout
+     Semantics.DynamicValues
+     Semantics.Denotation
+     Semantics.MemoryAddress
+     Semantics.LLVMEvents
+     Handlers.FiniteMemory.
+
+Require Import Ceres.Ceres.
+
+Import MonadNotation.
+Import EqvNotation.
+Import ListNotations.
+
+Set Implicit Arguments.
+Set Contextual Implicit.
+
+#[local] Open Scope Z_scope.
+(* end hide *)
+
+(** * Memory Model: Theory
+    Reasoning principles for VIR's main memory model.
+*)
+
+Import FinSizeof.
+
+Module Type MEMORY_THEORY (LLVMEvents : LLVM_INTERACTIONS(Addr)).
+  (** ** Theory of the general operations over the finite maps we manipulate *)
+  Import LLVMEvents.
+  Import DV.
+  Open Scope list.
+
+  Module Mem := FiniteMemory.Make(LLVMEvents).
+  Export Mem.
+
+  (* TODO: move this? *)
+  Definition ErrSID_evals_to {A} (e : ErrSID A) sid pr (x : A) : Prop
+    := evalErrSID e sid pr = inr (inr x).
+
+  (* TODO: move this? *)
+  Definition ErrSID_runs_to {A} (e : ErrSID A) sid pr (x : A) sid' pr': Prop
+    := runErrSID e sid pr = (inr (inr x), sid', pr').
+
+  Definition ErrSID_MemState_runs_to (e : MemState -> ErrSID memory_stack) (m m' : MemState) : Prop
+    := runErrSID (e m) (ms_sid m) (ms_prov m) = (inr (inr (ms_memory_stack m')), ms_sid m', ms_prov m').
+
+  Definition ErrSID_MemState_ms_runs_to (e : memory_stack -> ErrSID memory_stack) (m m' : MemState) : Prop
+    := runErrSID (e (ms_memory_stack m)) (ms_sid m) (ms_prov m) = (inr (inr (ms_memory_stack m')), ms_sid m', ms_prov m').
+
+
+Section Serialization_Theory.
+
+  Variable endianess : Endianess.
+  (** Length properties *)
+
+  Lemma length_bytes_of_int:
+    forall n x, List.length (bytes_of_int endianess n x) = n.
+  Proof.
+    destruct endianess.
+    - induction n; cbn; intros; auto.
+      rewrite app_length.
+      cbn in IHn.
+      cbn.
+      rewrite IHn.
+      lia.
+    - induction n; simpl; intros; auto.
+  Qed.
+
+  (* The relation defining serializable dvalues. *)
+  Inductive serialize_defined : dvalue -> Prop :=
+  | d_addr: forall addr,
+      serialize_defined (DVALUE_Addr addr)
+  | d_i1: forall i1,
+      serialize_defined (DVALUE_I1 i1)
+  | d_i8: forall i1,
+      serialize_defined (DVALUE_I8 i1)
+  | d_i32: forall i32,
+      serialize_defined (DVALUE_I32 i32)
+  | d_i64: forall i64,
+      serialize_defined (DVALUE_I64 i64)
+  | d_struct_empty:
+      serialize_defined (DVALUE_Struct [])
+  | d_struct_nonempty: forall dval fields_list,
+      serialize_defined dval ->
+      serialize_defined (DVALUE_Struct fields_list) ->
+      serialize_defined (DVALUE_Struct (dval :: fields_list))
+  | d_array_empty:
+      serialize_defined (DVALUE_Array [])
+  | d_array_nonempty: forall dval fields_list,
+      serialize_defined dval ->
+      serialize_defined (DVALUE_Array fields_list) ->
+      serialize_defined (DVALUE_Array (dval :: fields_list)).
+
+  Lemma fold_sizeof :
+    forall (dts : list dtyp) n,
+      (fold_left (fun (acc : N) (x : dtyp) => acc + sizeof_dtyp x) dts n =
+      n + fold_left (fun (acc : N) (x : dtyp) => acc + sizeof_dtyp x) dts 0)%N.
+  Proof.
+    induction dts; intros n.
+    - cbn. rewrite N.add_0_r. reflexivity.
+    - cbn. rewrite IHdts at 1. rewrite (IHdts (sizeof_dtyp a)).
+      rewrite N.add_assoc.
+      reflexivity.
+  Qed.
+
+  Lemma sizeof_struct_cons :
+    forall dt dts,
+      (sizeof_dtyp (DTYPE_Struct (dt :: dts)) = sizeof_dtyp dt + sizeof_dtyp (DTYPE_Struct dts))%N.
+  Proof.
+    cbn.
+    intros dt dts.
+    rewrite fold_sizeof. reflexivity.
+  Qed.
+
+  Lemma sizeof_packed_struct_cons :
+    forall dt dts,
+      (sizeof_dtyp (DTYPE_Packed_struct (dt :: dts)) = sizeof_dtyp dt + sizeof_dtyp (DTYPE_Packed_struct dts))%N.
+  Proof.
+    cbn.
+    intros dt dts.
+    rewrite fold_sizeof. reflexivity.
+  Qed.
+
+  Lemma sizeof_dvalue_pos :
+    forall dt,
+      (0 <= sizeof_dtyp dt)%N.
+  Proof.
+    intros dt.
+    lia.
+  Qed.
+
+  (* Lemma sizeof_serialized : *)
+  (*   forall uv dt, *)
+  (*     uvalue_has_dtyp uv dt -> *)
+  (*     N.of_nat (List.length (serialize_sbytes uv)) = sizeof_dtyp dt. *)
+  (* Proof. *)
+  (*   intros dv dt TYP. *)
+  (*   induction TYP; try solve [cbn; auto]. *)
+  (*   - cbn. rewrite DynamicValues.unsupported_cases_match; auto. *)
+  (*   - cbn. *)
+  (*     rewrite app_length. *)
+  (*     rewrite Nnat.Nat2N.inj_add. *)
+  (*     rewrite IHTYP1. *)
+  (*     cbn in IHTYP2. rewrite IHTYP2. *)
+  (*     symmetry. *)
+  (*     apply fold_sizeof. *)
+  (*   - cbn. *)
+  (*     rewrite app_length. *)
+  (*     rewrite Nnat.Nat2N.inj_add. *)
+  (*     rewrite IHTYP1. *)
+  (*     cbn in IHTYP2. rewrite IHTYP2. *)
+  (*     symmetry. *)
+  (*     apply fold_sizeof. *)
+  (*   - generalize dependent sz. *)
+  (*     induction xs; intros sz H; cbn. *)
+  (*     + subst; auto. *)
+  (*     + cbn in *. rewrite <- H. rewrite app_length. *)
+  (*       replace (N.of_nat (S (Datatypes.length xs)) * sizeof_dtyp dt)%N *)
+  (*         with (sizeof_dtyp dt + N.of_nat (Datatypes.length xs) * sizeof_dtyp dt)%N. *)
+  (*       * rewrite Nnat.Nat2N.inj_add. rewrite IHxs with (sz:=Datatypes.length xs); auto. *)
+  (*         apply N.add_cancel_r; auto. *)
+  (*       * rewrite Nnat.Nat2N.inj_succ. rewrite N.mul_succ_l. lia. *)
+  (*   - generalize dependent sz. *)
+  (*     induction xs; intros sz H; cbn. *)
+  (*     + subst; auto. *)
+  (*     + cbn in *. rewrite <- H. rewrite app_length. *)
+  (*       replace (N.of_nat (S (Datatypes.length xs)) * sizeof_dtyp dt)%N *)
+  (*         with (sizeof_dtyp dt + N.of_nat (Datatypes.length xs) * sizeof_dtyp dt)%N. *)
+  (*       * rewrite Nnat.Nat2N.inj_add. rewrite IHxs with (sz:=Datatypes.length xs); auto. *)
+  (*         apply N.add_cancel_r; auto. *)
+  (*       * rewrite Nnat.Nat2N.inj_succ. rewrite N.mul_succ_l. lia. *)
+  (* Qed. *)
+
+  (* Lemma firstn_sizeof_dtyp : *)
+  (*   forall dv dt, *)
+  (*     dvalue_has_dtyp dv dt -> *)
+  (*     (firstn (N.to_nat (sizeof_dtyp dt)) (serialize_dvalue dv)) = serialize_dvalue dv. *)
+  (* Proof. *)
+  (*   intros dv dt TYP. *)
+  (*   induction TYP; auto. *)
+  (*   - cbn. rewrite DynamicValues.unsupported_cases_match. reflexivity. auto. *)
+  (*   - (* Structs *) *)
+  (*     rewrite sizeof_struct_cons. *)
+  (*     cbn. *)
+  (*     rewrite <- sizeof_serialized with (dv:=f); auto. *)
+
+  (*     replace (N.to_nat *)
+  (*                (N.of_nat (Datatypes.length (serialize_dvalue f)) + *)
+  (*                 fold_left (fun (x : N) (acc : dtyp) => x + sizeof_dtyp acc) dts 0))%N with *)
+  (*         (Datatypes.length (serialize_dvalue f) + *)
+  (*          N.to_nat (fold_left (fun (x : N) (acc : dtyp) => (x + sizeof_dtyp acc)%N) dts 0%N))%nat. *)
+  (*     + rewrite firstn_app_2. *)
+  (*       cbn in *. *)
+  (*       rewrite IHTYP2. *)
+  (*       reflexivity. *)
+  (*     + rewrite Nnat.N2Nat.inj_add; try lia. *)
+  (*   - (* Packed Structs *) *)
+  (*     rewrite sizeof_packed_struct_cons. *)
+  (*     cbn. *)
+  (*     rewrite <- sizeof_serialized with (dv:=f); auto. *)
+
+  (*     replace (N.to_nat *)
+  (*                (N.of_nat (Datatypes.length (serialize_dvalue f)) + *)
+  (*                 fold_left (fun (x : N) (acc : dtyp) => x + sizeof_dtyp acc) dts 0))%N with *)
+  (*         (Datatypes.length (serialize_dvalue f) + *)
+  (*          N.to_nat (fold_left (fun (x : N) (acc : dtyp) => (x + sizeof_dtyp acc)%N) dts 0%N))%nat. *)
+  (*     + rewrite firstn_app_2. *)
+  (*       cbn in *. *)
+  (*       rewrite IHTYP2. *)
+  (*       reflexivity. *)
+  (*     + rewrite Nnat.N2Nat.inj_add; try lia. *)
+  (*   - (* Arrays *) *)
+  (*     generalize dependent sz. *)
+  (*     induction xs; intros sz H. *)
+  (*     + cbn. apply firstn_nil. *)
+  (*     + cbn in *. inversion H. *)
+  (*       replace (N.of_nat (S (Datatypes.length xs)) * sizeof_dtyp dt)%N with *)
+  (*           (sizeof_dtyp dt + N.of_nat (Datatypes.length xs) * sizeof_dtyp dt)%N. *)
+  (*       * rewrite Nnat.N2Nat.inj_add. *)
+  (*         -- cbn. rewrite <- sizeof_serialized with (dv:=a). *)
+  (*            rewrite Nnat.Nat2N.id. *)
+  (*            rewrite firstn_app_2. *)
+  (*            rewrite sizeof_serialized with (dt:=dt). *)
+  (*            apply app_prefix. *)
+  (*            apply IHxs. *)
+  (*            intros x Hin. *)
+  (*            apply IH; intuition. *)
+  (*            intros x Hin; auto. *)
+  (*            auto. *)
+  (*            auto. *)
+  (*            auto. *)
+  (*       * rewrite Nnat.Nat2N.inj_succ. rewrite N.mul_succ_l. lia. *)
+  (*   - (* Vectors *) *)
+  (*     generalize dependent sz. *)
+  (*     induction xs; intros sz H. *)
+  (*     + cbn. apply firstn_nil. *)
+  (*     + cbn in *. inversion H. *)
+  (*       replace (N.of_nat (S (Datatypes.length xs)) * sizeof_dtyp dt)%N with *)
+  (*           (sizeof_dtyp dt + N.of_nat (Datatypes.length xs) * sizeof_dtyp dt)%N. *)
+  (*       * rewrite Nnat.N2Nat.inj_add. *)
+  (*         -- cbn. rewrite <- sizeof_serialized with (dv:=a). *)
+  (*            rewrite Nnat.Nat2N.id. *)
+  (*            rewrite firstn_app_2. *)
+  (*            rewrite sizeof_serialized with (dt:=dt). *)
+  (*            apply app_prefix. *)
+  (*            apply IHxs. *)
+  (*            intros x Hin. *)
+  (*            apply IH; intuition. *)
+  (*            intros x Hin; auto. *)
+  (*            auto. *)
+  (*            auto. *)
+  (*            auto. *)
+  (*       * rewrite Nnat.Nat2N.inj_succ. rewrite N.mul_succ_l. lia. *)
+  (* Qed. *)
+
+  (* Lemma all_not_sundef_cons : *)
+  (*   forall b bs, *)
+  (*     all_not_sundef (b :: bs) = true -> *)
+  (*     all_not_sundef bs = true. *)
+  (* Proof. *)
+  (*   intros b bs H. *)
+  (*   cbn in H. *)
+  (*   unfold all_not_sundef. *)
+  (*   apply andb_prop in H as [Hid Hall]. *)
+  (*   auto. *)
+  (* Qed. *)
+
+  (* Lemma all_not_sundef_app : *)
+  (*   forall xs ys, *)
+  (*     all_not_sundef xs -> *)
+  (*     all_not_sundef ys -> *)
+  (*     all_not_sundef (xs ++ ys). *)
+  (* Proof. *)
+  (*   induction xs; intros ys Hxs Hys; auto. *)
+  (*   cbn in *. *)
+  (*   apply andb_prop in Hxs. *)
+  (*   apply andb_true_iff. *)
+  (*   intuition. *)
+  (*   apply IHxs; auto. *)
+  (* Qed. *)
+
+  (* Hint Resolve all_not_sundef_app: core. *)
+
+  (* Lemma byte_defined : *)
+  (*   forall b bs, *)
+  (*     all_not_sundef bs -> *)
+  (*     In b bs -> *)
+  (*     Sbyte_defined b. *)
+  (* Proof. *)
+  (*   intros b bs Hundef Hin. *)
+  (*   induction bs. *)
+  (*   - inversion Hin. *)
+  (*   - apply andb_prop in Hundef as [Hid Hall]. *)
+  (*     inversion Hin; subst. *)
+  (*     + apply Hid. *)
+  (*     + apply IHbs; auto. *)
+  (* Qed. *)
+
+  (* Lemma dvalue_serialized_not_sundef : *)
+  (*   forall dv, *)
+  (*     all_not_sundef (serialize_dvalue dv) = true. *)
+  (* Proof. *)
+  (*   intros dv. *)
+  (*   induction dv; auto. *)
+  (*   - induction fields. *)
+  (*     + reflexivity. *)
+  (*     + cbn. apply forallb_forall. *)
+  (*       intros x Hin. *)
+  (*       apply list_in_map_inv in Hin as [b [Hxb Hin]]; subst. *)
+  (*       apply in_app_or in Hin as [Hin | Hin]. *)
+  (*       * assert (In a (a :: fields)) as Hina by intuition. *)
+  (*         specialize (H a Hina). *)
+  (*         eapply byte_defined; eauto. *)
+  (*       * assert (forall u : dvalue, In u fields -> all_not_sundef (serialize_dvalue u) = true) as Hu. *)
+  (*         intros u Hinu. *)
+  (*         apply H. cbn. auto. *)
+
+  (*         specialize (IHfields Hu). *)
+  (*         eapply byte_defined. apply IHfields. *)
+  (*         apply Hin. *)
+  (*   - induction fields. *)
+  (*     + reflexivity. *)
+  (*     + cbn. apply forallb_forall. *)
+  (*       intros x Hin. *)
+  (*       apply list_in_map_inv in Hin as [b [Hxb Hin]]; subst. *)
+  (*       apply in_app_or in Hin as [Hin | Hin]. *)
+  (*       * assert (In a (a :: fields)) as Hina by intuition. *)
+  (*         specialize (H a Hina). *)
+  (*         eapply byte_defined; eauto. *)
+  (*       * assert (forall u : dvalue, In u fields -> all_not_sundef (serialize_dvalue u) = true) as Hu. *)
+  (*         intros u Hinu. *)
+  (*         apply H. cbn. auto. *)
+
+  (*         specialize (IHfields Hu). *)
+  (*         eapply byte_defined. apply IHfields. *)
+  (*         apply Hin. *)
+  (*   - induction elts. *)
+  (*     + reflexivity. *)
+  (*     + cbn in *. *)
+  (*       rewrite map_app. *)
+  (*       rewrite forallb_app. *)
+  (*       apply andb_true_iff. *)
+  (*       split. *)
+  (*       * apply H; auto. *)
+  (*       * apply IHelts. intros e H0. *)
+  (*         apply H; auto. *)
+  (*   - induction elts. *)
+  (*     + reflexivity. *)
+  (*     + cbn in *. *)
+  (*       rewrite map_app. *)
+  (*       rewrite forallb_app. *)
+  (*       apply andb_true_iff. *)
+  (*       split. *)
+  (*       * apply H; auto. *)
+  (*       * apply IHelts. intros e H0. *)
+  (*         apply H; auto. *)
+  (* Qed. *)
+
+  (* Hint Resolve dvalue_serialized_not_sundef: core. *)
+
+  (* Lemma all_not_sundef_fold_right_serialize : *)
+  (*   forall xs, *)
+  (*     all_not_sundef (fold_right (fun (dv : dvalue) (acc : list SByte) => serialize_dvalue dv ++ acc) [ ] xs). *)
+  (* Proof. *)
+  (*   induction xs; auto. *)
+  (*   - cbn. apply all_not_sundef_app; auto. *)
+  (* Qed. *)
+
+  (* Hint Resolve all_not_sundef_fold_right_serialize: core. *)
+
+  (* Lemma all_not_sundef_deserialized : *)
+  (*   forall bs t, *)
+  (*     all_not_sundef bs -> *)
+  (*     deserialize_sbytes_defined bs t = deserialize_sbytes bs t. *)
+  (* Proof. *)
+  (*   intros bs t H. *)
+  (*   unfold deserialize_sbytes. *)
+  (*   rewrite H. *)
+  (*   auto. *)
+  (* Qed. *)
+
+  (* Lemma deserialize_sbytes_defined_dvalue : *)
+  (*   forall dv t, *)
+  (*     deserialize_sbytes_defined (serialize_dvalue dv) t = deserialize_sbytes (serialize_dvalue dv) t. *)
+  (* Proof. *)
+  (*   intros dv t. *)
+  (*   apply all_not_sundef_deserialized. *)
+  (*   apply dvalue_serialized_not_sundef. *)
+  (* Qed. *)
+
+  (* Hint Resolve deserialize_sbytes_defined: core. *)
+
+  (* Lemma serialize_firstn_app : *)
+  (*   forall dv dt rest, *)
+  (*     dvalue_has_dtyp dv dt -> *)
+  (*     firstn (N.to_nat (sizeof_dtyp dt)) *)
+  (*            (serialize_dvalue dv ++ rest) = serialize_dvalue dv. *)
+  (* Proof. *)
+  (*   intros dv dt rest H. *)
+  (*   erewrite <- sizeof_serialized; eauto. *)
+  (*   rewrite Nnat.Nat2N.id. *)
+  (*   rewrite firstn_app. *)
+  (*   rewrite Nat.sub_diag. *)
+  (*   cbn. *)
+  (*   rewrite app_nil_r. *)
+  (*   rewrite <- (Nnat.Nat2N.id (Datatypes.length (serialize_dvalue dv))). *)
+  (*   erewrite sizeof_serialized; eauto. *)
+  (*   rewrite firstn_sizeof_dtyp; eauto. *)
+  (* Qed. *)
+
+  (* Lemma serialize_skipn_app : *)
+  (*   forall dv dt rest, *)
+  (*     dvalue_has_dtyp dv dt -> *)
+  (*     skipn (N.to_nat (sizeof_dtyp dt)) *)
+  (*           (serialize_dvalue dv ++ rest) = rest. *)
+  (* Proof. *)
+  (*   intros dv dt rest H. *)
+  (*   erewrite <- sizeof_serialized; eauto. *)
+  (*   rewrite Nnat.Nat2N.id. *)
+  (*   apply skipn_length_app. *)
+  (* Qed. *)
+
+  (* Lemma serialize_fold_length : *)
+  (*   forall xs dt, *)
+  (*     (forall x, In x xs -> dvalue_has_dtyp x dt) -> *)
+  (*     N.to_nat (N.of_nat (Datatypes.length xs) * sizeof_dtyp dt) = *)
+  (*     Datatypes.length *)
+  (*       (fold_right (fun (dv : dvalue) (acc : list SByte) => serialize_dvalue dv ++ acc) [] xs). *)
+  (* Proof. *)
+  (*   induction xs; intros dt H; auto. *)
+
+  (*   cbn. *)
+  (*   rewrite app_length. *)
+  (*   apply Nnat.Nat2N.inj. *)
+  (*   rewrite Nnat.N2Nat.id. *)
+  (*   rewrite Nnat.Nat2N.inj_add. *)
+
+  (*   break_match. *)
+  (*   - erewrite sizeof_serialized; intuition. *)
+
+  (*     rewrite Heqn. cbn. *)
+  (*     erewrite <- IHxs; intuition. *)
+  (*     lia. *)
+  (*   - erewrite sizeof_serialized; intuition. *)
+
+  (*     rewrite Heqn. cbn. *)
+  (*     erewrite <- IHxs; intuition. *)
+  (*     rewrite Nnat.N2Nat.id. *)
+  (*     break_match; lia. *)
+  (* Qed. *)
+
+
+End Serialization_Theory.
+
+Section Memory_Stack_Theory.
+
+  Lemma not_overlaps__no_overlap :
+    forall a1 τ1 a2 τ2,
+      ~ overlaps_dtyp a1 τ1 a2 τ2 ->
+      no_overlap_dtyp a1 τ1 a2 τ2.
+  Proof.
+    intros [a1_r a1_o] τ1 [a2_r a2_o] τ2 H.
+    unfold overlaps_dtyp, overlaps in H.
+    unfold no_overlap_dtyp, no_overlap.
+    lia.
+  Qed.
+
+  Lemma no_overlap__not_overlaps :
+    forall a1 τ1 a2 τ2,
+      no_overlap_dtyp a1 τ1 a2 τ2 ->
+      ~ overlaps_dtyp a1 τ1 a2 τ2.
+  Proof.
+    intros [a1_r a1_o] τ1 [a2_r a2_o] τ2 H.
+    unfold no_overlap_dtyp, no_overlap in H.
+    unfold overlaps_dtyp, overlaps.
+    lia.
+  Qed.
+
+  Lemma no_overlap_dec :
+    forall ptr1 ptr2 s1 s2,
+      {no_overlap ptr1 s1 ptr2 s2} + {~ (no_overlap ptr1 s1 ptr2 s2)}.
+  Proof.
+    intros [a1 pr1] [a2 pr2] s1 s2.
+    unfold no_overlap.
+    cbn.
+
+    destruct (Int.Z_as_Int.gt_le_dec (a1) (a2 + s2 - 1)).
+    { left. auto. }
+
+    destruct (Int.Z_as_Int.gt_le_dec (a2) (a1 + s1 - 1)).
+    { left. auto. }
+
+    right. intuition.
+  Qed.
+
+  Lemma no_overlap_dtyp_dec :
+    forall ptr1 ptr2 τ1 τ2,
+      {no_overlap_dtyp ptr1 τ1 ptr2 τ2} + {~ (no_overlap_dtyp ptr1 τ1 ptr2 τ2)}.
+  Proof.
+    intros ptr1 ptr2 τ1 τ2.
+    apply no_overlap_dec.
+  Qed.
+
+  Lemma gep_array_ptr_overlap_dtyp :
+    forall ptr ix (sz : N) τ elem_ptr,
+      DynamicValues.Int64.unsigned ix < Z.of_N sz -> (* Not super happy about this *)
+      (0 < sizeof_dtyp τ)%N ->
+      handle_gep_addr (DTYPE_Array sz τ) ptr
+                      [DVALUE_I64 (repr 0); DVALUE_I64 ix] = inr elem_ptr ->
+      ~(no_overlap_dtyp elem_ptr τ ptr (DTYPE_Array sz τ)).
+  Proof.
+    intros ptr ix sz τ elem_ptr BOUNDS SIZE GEP.
+    intros NO_OVER.
+    unfold no_overlap_dtyp, no_overlap in NO_OVER.
+
+    destruct ptr as [ptr_a prov].
+    destruct elem_ptr as [elem_ptr_b elem_ptr_i].
+
+    unfold handle_gep_addr in GEP.
+    cbn in *.
+    inversion GEP; subst.
+
+    destruct NO_OVER as [NO_OVER | NO_OVER].
+    - rewrite Integers.Int64.unsigned_repr in NO_OVER; [|cbn; lia].
+      replace (ptr_a + Z.of_N (sz * sizeof_dtyp τ) * 0 + DynamicValues.Int64.unsigned ix * Z.of_N (sizeof_dtyp τ)) with (ptr_a + DynamicValues.Int64.unsigned ix * Z.of_N (sizeof_dtyp τ)) in NO_OVER by lia.
+      pose proof (Int64.unsigned_range ix) as [? ?].
+      assert (Z.of_N sz > 0). lia.
+      rewrite N2Z.inj_mul in NO_OVER.
+      replace (ptr_a + Z.of_N sz * Z.of_N (sizeof_dtyp τ) - 1) with (ptr_a + (Z.of_N sz * Z.of_N (sizeof_dtyp τ) - 1)) in NO_OVER by lia.
+      apply Zorder.Zplus_gt_reg_l in NO_OVER.
+
+      assert (Z.of_N sz * Z.of_N (sizeof_dtyp τ) - Z.of_N (sizeof_dtyp τ) <= Z.of_N sz * Z.of_N (sizeof_dtyp τ) - 1).
+      lia.
+      assert (Int64.unsigned ix * Z.of_N (sizeof_dtyp τ) <= (Z.of_N sz - 1) * Z.of_N (sizeof_dtyp τ)).
+      { apply Zmult_le_compat_r; lia. }
+      lia.
+    - rewrite Integers.Int64.unsigned_repr in NO_OVER; [|cbn; lia].
+      replace (ptr_a + Z.of_N (sz * sizeof_dtyp τ) * 0 + DynamicValues.Int64.unsigned ix * Z.of_N (sizeof_dtyp τ)) with (ptr_a + DynamicValues.Int64.unsigned ix * Z.of_N (sizeof_dtyp τ)) in NO_OVER by lia.
+      pose proof (Int64.unsigned_range ix) as [? ?].
+      lia.
+  Qed.
+
+  Definition non_void (τ : dtyp) : Prop :=
+    τ <> DTYPE_Void.
+
+  (* TODO: Move this? *)
+  Lemma unsigned_I1_in_range : forall (x : DynamicValues.int1),
+      0 <= DynamicValues.Int1.unsigned x <= 1.
+  Proof.
+    destruct x as [x [? ?]].
+    cbn in *.
+    unfold DynamicValues.Int1.modulus,DynamicValues.Int1.wordsize, DynamicValues.Wordsize1.wordsize, two_power_nat in *.
+    cbn in *; lia.
+  Qed.
+
+  Lemma unsigned_I8_in_range : forall (x : DynamicValues.int8),
+      0 <= DynamicValues.Int8.unsigned x <= 255.
+  Proof.
+    destruct x as [x [? ?]].
+    cbn in *.
+    unfold DynamicValues.Int8.modulus,DynamicValues.Int8.wordsize, DynamicValues.Wordsize8.wordsize, two_power_nat in *.
+    cbn in *; lia.
+  Qed.
+
+  Lemma unsigned_I32_in_range : forall (x : DynamicValues.int32),
+      0 <= DynamicValues.Int32.unsigned x <= 4294967295.
+  Proof.
+    destruct x as [x [? ?]].
+    cbn in *.
+    unfold DynamicValues.Int32.modulus,DynamicValues.Int8.wordsize, DynamicValues.Wordsize8.wordsize, two_power_nat in *.
+    cbn in *; lia.
+  Qed.
+
+  Lemma unsigned_I64_in_range : forall (x : DynamicValues.int64),
+      0 <= DynamicValues.Int64.unsigned x <= 18446744073709551615.
+  Proof.
+    destruct x as [x [? ?]].
+    cbn in *.
+    unfold DynamicValues.Int32.modulus,DynamicValues.Int8.wordsize, Int64.modulus, DynamicValues.Wordsize8.wordsize, two_power_nat in *.
+    cbn in *;lia.
+  Qed.
+
+  Lemma Z_div_mod' :
+    forall a b q r : Z, b > 0 -> Z.div_eucl a b = (q, r) -> a = b * q + r /\ 0 <= r < b.
+  Proof.
+    intros.
+    pose proof (Z_div_mod a b H).
+    break_let.
+    congruence.
+  Qed.
+
+    (* CB TODO: Figure out where these predicates should live, or figure
+       out how to get rid of them. Currently not using some of these... *)
+
+    Definition not_pointer (τ : dtyp) : Prop
+      := τ <> DTYPE_Pointer.
+
+    Definition not_undef (v : uvalue) : Prop
+      := forall τ, v <> UVALUE_Undef τ.
+
+    Lemma div_add_lemma :
+      forall (x y d : Z),
+        0 <= y < d ->
+        (d * x + y) / d = x.
+    Proof.
+      intros x y d H.
+      rewrite Z.add_comm.
+      rewrite Z.mul_comm.
+      rewrite Z_div_plus.
+      rewrite Zdiv_small with (x:=y) by lia.
+      all: lia.
+    Qed.
+
+    Ltac destruct_div_eucls :=
+      repeat
+        match goal with
+        | H: Z.div_eucl _ _ = _ |- _ =>
+          apply Z_div_mod' in H; [destruct H|lia]
+        end.
+
+    Ltac rewrite_div_adds :=
+      repeat
+        match goal with
+        | H: context [(?d * ?x + ?z) / ?d] |- _ =>
+          rewrite div_add_lemma in H; [|lia]; subst
+        end.
+
+    Ltac unfold_lookup_all_index :=
+      rewrite <- N.succ_pos_pred;
+      match goal with
+      | |- context [N.succ (Pos.pred_N ?x)] =>
+        let var := fresh "var" in
+        set (var := Pos.pred_N x); cbn in var; subst var
+      end;
+      rewrite lookup_all_index_add.
+
+    Ltac unroll_lookup_all_index :=
+      simpl add_all_index; simpl sizeof_dtyp;
+      repeat unfold_lookup_all_index.
+
+    Ltac solve_integer_deserialize :=
+      unroll_lookup_all_index; cbn; f_equal;
+      match goal with
+      | |- _ = ?x =>
+        first [ pose proof (unsigned_I8_in_range x)
+              | pose proof (unsigned_I32_in_range x)
+              | pose proof (unsigned_I64_in_range x)
+              ];
+
+        repeat rewrite Byte.unsigned_repr_eq;
+        unfold Byte.max_unsigned, Byte.modulus, Byte.wordsize, Wordsize_8.wordsize;
+        cbn;
+        change (two_power_nat 8) with 256;
+        let xv := fresh "xv" in
+        let Hxv := fresh "Hxv" in
+        first [ remember (Int8.unsigned x) as xv eqn:Hxv
+              | remember (Int32.unsigned x) as xv eqn:Hxv
+              | remember (Int64.unsigned x) as xv eqn:Hxv
+              ];
+        match goal with
+        | [|- context[Int8.repr ?zv]] => replace zv with xv
+        | [|- context[Int32.repr ?zv]] => replace zv with xv
+        | [|- context[Int64.repr ?zv]] => replace zv with xv
+        end;
+        [subst xv;
+         try solve [ apply Int1.repr_unsigned
+                   | apply Int8.repr_unsigned
+                   | apply Int32.repr_unsigned
+                   | apply Int64.repr_unsigned
+                   ]
+        |];
+        clear Hxv;
+        unfold Z.modulo;
+        repeat break_let;
+        destruct_div_eucls;
+        subst;
+        rewrite_div_adds;
+        lia
+      end.
+
+    (* Lemma deserialize_sbytes_dvalue_all_not_sundef : *)
+    (*   forall dv dt bytes, *)
+    (*     deserialize_sbytes bytes dt = dvalue_to_uvalue dv -> *)
+    (*     all_not_sundef bytes = true. *)
+    (* Proof. *)
+    (*   intros dv dt bytes DES. *)
+    (*   unfold deserialize_sbytes in DES. *)
+    (*   break_match_hyp; auto. *)
+
+    (*   destruct dv; inversion DES. *)
+    (* Qed. *)
+
+    (* Lemma deserialize_struct_element : *)
+    (*   forall f fields ft fts f_bytes fields_bytes, *)
+    (*     is_supported (DTYPE_Struct (ft :: fts)) -> *)
+    (*     all_not_sundef f_bytes = true -> *)
+    (*     all_not_sundef fields_bytes = true -> *)
+    (*     N.to_nat (sizeof_dtyp ft) = Datatypes.length f_bytes -> *)
+    (*     deserialize_sbytes f_bytes ft = f -> *)
+    (*     deserialize_sbytes fields_bytes (DTYPE_Struct fts) = UVALUE_Struct fields -> *)
+    (*     deserialize_sbytes (f_bytes ++ fields_bytes) (DTYPE_Struct (ft :: fts)) = *)
+    (*     UVALUE_Struct (f :: fields). *)
+    (* Proof. *)
+    (*   intros f fields ft fts. *)
+    (*   generalize dependent ft. *)
+    (*   generalize dependent fields. *)
+    (*   generalize dependent f. *)
+    (*   induction fts; intros f fields ft f_bytes fields_bytes SUP UNDEF_BYTES UNDEF_FIELDS SIZE FIELD FIELDS. *)
+
+    (*   - rewrite <- all_not_sundef_deserialized in FIELD; auto. *)
+    (*     rewrite <- all_not_sundef_deserialized in FIELDS; auto. *)
+    (*     rewrite <- all_not_sundef_deserialized; auto using all_not_sundef_app. *)
+
+    (*     cbn in FIELDS; inversion FIELDS; subst; cbn. *)
+
+    (*     replace (N.to_nat (sizeof_dtyp ft)) with (Datatypes.length f_bytes + 0)%nat by lia. *)
+    (*     rewrite firstn_app_2; cbn. *)
+    (*     rewrite app_nil_r. *)
+
+    (*     congruence. *)
+    (*   - rewrite <- all_not_sundef_deserialized in FIELD; auto. *)
+    (*     rewrite <- all_not_sundef_deserialized in FIELDS; auto. *)
+    (*     rewrite <- all_not_sundef_deserialized; auto using all_not_sundef_app. *)
+
+    (*     cbn in FIELDS; inversion FIELDS; subst; cbn. *)
+        
+    (*     replace (N.to_nat (sizeof_dtyp ft)) with (Datatypes.length f_bytes + 0)%nat by lia. *)
+    (*     rewrite firstn_app_2; cbn. *)
+    (*     rewrite app_nil_r. *)
+
+    (*     do 2 f_equal. *)
+
+    (*     replace (Datatypes.length f_bytes + 0)%nat with (Datatypes.length f_bytes) by lia. *)
+    (*     rewrite skipn_length_app. *)
+    (*     congruence. *)
+    (* Qed. *)
+
+    (* Lemma deserialize_packed_struct_element : *)
+    (*   forall f fields ft fts f_bytes fields_bytes, *)
+    (*     is_supported (DTYPE_Packed_struct (ft :: fts)) -> *)
+    (*     all_not_sundef f_bytes = true -> *)
+    (*     all_not_sundef fields_bytes = true -> *)
+    (*     N.to_nat (sizeof_dtyp ft) = Datatypes.length f_bytes -> *)
+    (*     deserialize_sbytes f_bytes ft = f -> *)
+    (*     deserialize_sbytes fields_bytes (DTYPE_Packed_struct fts) = UVALUE_Packed_struct fields -> *)
+    (*     deserialize_sbytes (f_bytes ++ fields_bytes) (DTYPE_Packed_struct (ft :: fts)) = *)
+    (*     UVALUE_Packed_struct (f :: fields). *)
+    (* Proof. *)
+    (*   intros f fields ft fts. *)
+    (*   generalize dependent ft. *)
+    (*   generalize dependent fields. *)
+    (*   generalize dependent f. *)
+    (*   induction fts; intros f fields ft f_bytes fields_bytes SUP UNDEF_BYTES UNDEF_FIELDS SIZE FIELD FIELDS. *)
+
+    (*   - rewrite <- all_not_sundef_deserialized in FIELD; auto. *)
+    (*     rewrite <- all_not_sundef_deserialized in FIELDS; auto. *)
+    (*     rewrite <- all_not_sundef_deserialized; auto using all_not_sundef_app. *)
+
+    (*     cbn in FIELDS; inversion FIELDS; subst; cbn. *)
+
+    (*     replace (N.to_nat (sizeof_dtyp ft)) with (Datatypes.length f_bytes + 0)%nat by lia. *)
+    (*     rewrite firstn_app_2; cbn. *)
+    (*     rewrite app_nil_r. *)
+
+    (*     congruence. *)
+    (*   - rewrite <- all_not_sundef_deserialized in FIELD; auto. *)
+    (*     rewrite <- all_not_sundef_deserialized in FIELDS; auto. *)
+    (*     rewrite <- all_not_sundef_deserialized; auto using all_not_sundef_app. *)
+
+    (*     cbn in FIELDS; inversion FIELDS; subst; cbn. *)
+        
+    (*     replace (N.to_nat (sizeof_dtyp ft)) with (Datatypes.length f_bytes + 0)%nat by lia. *)
+    (*     rewrite firstn_app_2; cbn. *)
+    (*     rewrite app_nil_r. *)
+
+    (*     do 2 f_equal. *)
+
+    (*     replace (Datatypes.length f_bytes + 0)%nat with (Datatypes.length f_bytes) by lia. *)
+    (*     rewrite skipn_length_app. *)
+    (*     congruence. *)
+    (* Qed. *)
+
+    (* Lemma deserialize_array_element : *)
+    (*   forall sz elt elts ft elt_bytes elts_bytes, *)
+    (*     is_supported (DTYPE_Array sz ft) -> *)
+    (*     all_not_sundef elt_bytes = true -> *)
+    (*     all_not_sundef elts_bytes = true -> *)
+    (*     N.to_nat (sizeof_dtyp ft) = Datatypes.length elt_bytes -> *)
+    (*     deserialize_sbytes elt_bytes ft = elt -> *)
+    (*     deserialize_sbytes elts_bytes (DTYPE_Array sz ft) = UVALUE_Array elts -> *)
+    (*     deserialize_sbytes (elt_bytes ++ elts_bytes) (DTYPE_Array (N.succ sz) ft) = *)
+    (*     UVALUE_Array (elt :: elts). *)
+    (* Proof. *)
+    (*   induction sz; *)
+    (*     intros elt elts ft elt_bytes elts_bytes SUP UNDEF_BYTES UNDEF_ELTS SIZE ELT ELTS. *)
+      
+    (*   - rewrite <- all_not_sundef_deserialized in ELT; auto. *)
+    (*     rewrite <- all_not_sundef_deserialized in ELTS; auto. *)
+    (*     rewrite <- all_not_sundef_deserialized; auto using all_not_sundef_app. *)
+
+    (*     cbn in ELTS; inversion ELTS; subst; cbn. *)
+
+    (*     replace (N.to_nat (sizeof_dtyp ft)) with (Datatypes.length elt_bytes + 0)%nat by lia. *)
+    (*     rewrite Pos2Nat.inj_1. *)
+    (*     rewrite firstn_app_2; cbn. *)
+    (*     rewrite app_nil_r. *)
+
+    (*     congruence. *)
+    (*   - rewrite <- all_not_sundef_deserialized in ELT; auto. *)
+    (*     rewrite <- all_not_sundef_deserialized in ELTS; auto. *)
+    (*     rewrite <- all_not_sundef_deserialized; auto using all_not_sundef_app. *)
+
+    (*     cbn in ELTS; inversion ELTS; subst; cbn. *)
+        
+    (*     replace (N.to_nat (sizeof_dtyp ft)) with (Datatypes.length elt_bytes + 0)%nat by lia. *)
+    (*     rewrite Pos2Nat.inj_succ. *)
+    (*     rewrite firstn_app_2; cbn. *)
+    (*     rewrite app_nil_r. *)
+
+    (*     do 2 f_equal. *)
+
+    (*     replace (Datatypes.length elt_bytes + 0)%nat with (Datatypes.length elt_bytes) by lia. *)
+    (*     rewrite skipn_length_app. *)
+    (*     congruence. *)
+    (* Qed. *)
+
+    (* Lemma deserialize_vector_element : *)
+    (*   forall sz elt elts ft elt_bytes elts_bytes, *)
+    (*     is_supported (DTYPE_Vector sz ft) -> *)
+    (*     all_not_sundef elt_bytes = true -> *)
+    (*     all_not_sundef elts_bytes = true -> *)
+    (*     N.to_nat (sizeof_dtyp ft) = Datatypes.length elt_bytes -> *)
+    (*     deserialize_sbytes elt_bytes ft = elt -> *)
+    (*     deserialize_sbytes elts_bytes (DTYPE_Vector sz ft) = UVALUE_Vector elts -> *)
+    (*     deserialize_sbytes (elt_bytes ++ elts_bytes) (DTYPE_Vector (N.succ sz) ft) = *)
+    (*     UVALUE_Vector (elt :: elts). *)
+    (* Proof. *)
+    (*   induction sz; *)
+    (*     intros elt elts ft elt_bytes elts_bytes SUP UNDEF_BYTES UNDEF_ELTS SIZE ELT ELTS. *)
+      
+    (*   - rewrite <- all_not_sundef_deserialized in ELT; auto. *)
+    (*     rewrite <- all_not_sundef_deserialized in ELTS; auto. *)
+    (*     rewrite <- all_not_sundef_deserialized; auto using all_not_sundef_app. *)
+
+    (*     cbn in ELTS; inversion ELTS; subst; cbn. *)
+
+    (*     replace (N.to_nat (sizeof_dtyp ft)) with (Datatypes.length elt_bytes + 0)%nat by lia. *)
+    (*     rewrite Pos2Nat.inj_1. *)
+    (*     rewrite firstn_app_2; cbn. *)
+    (*     rewrite app_nil_r. *)
+
+    (*     congruence. *)
+    (*   - rewrite <- all_not_sundef_deserialized in ELT; auto. *)
+    (*     rewrite <- all_not_sundef_deserialized in ELTS; auto. *)
+    (*     rewrite <- all_not_sundef_deserialized; auto using all_not_sundef_app. *)
+
+    (*     cbn in ELTS; inversion ELTS; subst; cbn. *)
+        
+    (*     replace (N.to_nat (sizeof_dtyp ft)) with (Datatypes.length elt_bytes + 0)%nat by lia. *)
+    (*     rewrite Pos2Nat.inj_succ. *)
+    (*     rewrite firstn_app_2; cbn. *)
+    (*     rewrite app_nil_r. *)
+
+    (*     do 2 f_equal. *)
+
+    (*     replace (Datatypes.length elt_bytes + 0)%nat with (Datatypes.length elt_bytes) by lia. *)
+    (*     rewrite skipn_length_app. *)
+    (*     congruence. *)
+    (* Qed. *)
+
+    (** ** Deserialize - Serialize
+        Starting from a dvalue [val] whose [dtyp] is [t], if:
+        1. we serialize [val], getting a [list SByte]
+        2. we add all these bytes to the memory block, starting from the position [off], getting back a new [mem_block] m'
+        3. we lookup in this new memory [m'] the indices starting from [off] for the size of [t], getting back a [list SByte]
+        4. we deserialize this final list of bytes
+        then we should get back the initial value [val], albeit injected into [uvalue].
+
+        The proof should go by induction over [TYP] I think, and rely on [lookup_all_index_add] notably.
+     *)
+    (* Lemma deserialize_serialize : forall val t (TYP : dvalue_has_dtyp val t), *)
+    (*     forall off (bytes : mem_block) (SUP : is_supported t), *)
+    (*       deserialize_sbytes (lookup_all_index off (sizeof_dtyp t) (add_all_index (serialize_dvalue val) off bytes) SUndef) t = dvalue_to_uvalue val. *)
+    (* Proof. *)
+    (*   induction 1; try auto; intros; *)
+    (*     match goal with *)
+    (*     | H: is_supported ?t |- _ => *)
+    (*       try solve [inversion H] *)
+    (*     end. *)
+    (*   - unroll_lookup_all_index; cbn; f_equal. *)
+    (*   - unroll_lookup_all_index; cbn; f_equal. *)
+    (*     pose proof (unsigned_I1_in_range x). *)
+    (*     assert (EQ :DynamicValues.Int1.unsigned x / 256 = 0). *)
+    (*     apply Z.div_small; lia. *)
+    (*     rewrite EQ. *)
+    (*     repeat rewrite Zdiv_0_l. *)
+    (*     repeat rewrite Byte.unsigned_repr. *)
+    (*     all: unfold Byte.max_unsigned, Byte.modulus; cbn; try lia. *)
+    (*     rewrite Z.add_0_r. *)
+    (*     apply DynamicValues.Int1.repr_unsigned. *)
+    (*   - solve_integer_deserialize. *)
+    (*   - solve_integer_deserialize. *)
+    (*   - solve_integer_deserialize. *)
+    (*   - inversion SUP; subst; *)
+    (*     exfalso; apply H; constructor. *)
+    (*   - unroll_lookup_all_index; cbn; f_equal. *)
+    (*     clear bytes off. *)
+    (*     remember (Float.to_bits x) as xb. *)
+    (*     pose proof (unsigned_I64_in_range xb). *)
+    (*     repeat rewrite Byte.unsigned_repr_eq. *)
+    (*     unfold Byte.modulus, Byte.wordsize, Wordsize_8.wordsize; cbn. *)
+    (*     replace (two_power_nat 8) with 256 by reflexivity. *)
+    (*     remember (Int64.unsigned xb) as xbv. *)
+    (*     match goal with *)
+    (*     | [|- context[Int64.repr ?zv]] => replace zv with xbv *)
+    (*     end. *)
+    (*     + *)
+    (*       subst. *)
+    (*       rewrite Int64.repr_unsigned. *)
+    (*       apply Float.of_to_bits. *)
+    (*     + *)
+    (*       (* this is the same goal as I64 branch! *) *)
+    (*       clear -H. *)
+    (*       rewrite Z.add_0_r. *)
+    (*       unfold Z.modulo. *)
+    (*       repeat break_let. *)
+    (*       repeat match goal with *)
+    (*              | [H : Z.div_eucl _ _ = _ |- _] => apply Z_div_mod' in H; [destruct H | lia] *)
+    (*              end. *)
+    (*       subst. *)
+    (*       repeat *)
+    (*         match goal with *)
+    (*         | H: context [(?d * ?x + ?z) / ?d] |- _ => *)
+    (*           rewrite div_add_lemma in H; [|lia]; subst *)
+    (*         end. *)
+    (*       lia. *)
+    (*   - unroll_lookup_all_index; cbn; f_equal. *)
+    (*     clear bytes off. *)
+    (*     remember (Float32.to_bits x) as xb. *)
+    (*     pose proof (unsigned_I32_in_range xb). *)
+    (*     repeat rewrite Byte.unsigned_repr_eq. *)
+    (*     unfold Byte.modulus, Byte.wordsize, Wordsize_8.wordsize; cbn. *)
+    (*     replace (two_power_nat 8) with 256 by reflexivity. *)
+    (*     remember (Int32.unsigned xb) as xbv. *)
+    (*     match goal with *)
+    (*     | [|- context[Int32.repr ?zv]] => replace zv with xbv *)
+    (*     end. *)
+    (*     + *)
+    (*       subst. *)
+    (*       rewrite Int32.repr_unsigned. *)
+    (*       apply Float32.of_to_bits. *)
+    (*     + *)
+    (*       clear -H. *)
+
+    (*       rewrite Z.add_0_r. *)
+    (*       unfold Z.modulo. *)
+    (*       repeat break_let. *)
+    (*       repeat match goal with *)
+    (*              | [H : Z.div_eucl _ _ = _ |- _] => apply Z_div_mod' in H; [destruct H | lia] *)
+    (*              end. *)
+    (*       subst. *)
+    (*       rewrite Z.add_comm, Z.mul_comm, Z_div_plus in * by lia. *)
+    (*       rewrite Zdiv_small with (x:=z0) in * by lia. *)
+    (*       rewrite Z.add_0_l in *. *)
+    (*       subst. *)
+    (*       rewrite Z.add_comm, Z.mul_comm, Z_div_plus in * by lia. *)
+    (*       rewrite Zdiv_small with (x:=z2) in * by lia. *)
+    (*       rewrite Z.add_0_l in *. *)
+    (*       subst. *)
+    (*       rewrite Z.add_comm, Z.mul_comm, Z_div_plus in * by lia. *)
+    (*       rewrite Zdiv_small with (x:=z4) in * by lia. *)
+    (*       rewrite Z.add_0_l in *. *)
+    (*       subst. *)
+    (*       lia. *)
+    (*   - (* Structs *) *)
+    (*     rewrite sizeof_struct_cons. *)
+
+    (*     inversion SUP. *)
+    (*     subst. *)
+    (*     rename H0 into FIELD_SUP. *)
+    (*     apply List.Forall_cons_iff in FIELD_SUP. *)
+    (*     destruct FIELD_SUP as [dt_SUP dts_SUP]. *)
+    (*     assert (is_supported (DTYPE_Struct dts)) as SUP_STRUCT by (constructor; auto). *)
+
+    (*     cbn. *)
+    (*     rewrite lookup_all_index_append; [|apply sizeof_serialized; auto]. *)
+
+    (*     erewrite deserialize_struct_element; auto. *)
+    (*     +  erewrite <- sizeof_serialized; eauto. *)
+    (*       rewrite lookup_all_index_add_all_index_same_length; eauto. *)
+
+    (*       apply dvalue_serialized_not_sundef. *)
+    (*     + pose proof deserialize_sbytes_dvalue_all_not_sundef (DVALUE_Struct fields) (DTYPE_Struct dts) (lookup_all_index (off + Z.of_N (sizeof_dtyp dt)) (sizeof_dtyp (DTYPE_Struct dts)) *)
+    (*                                                                                                                       (add_all_index (serialize_dvalue (DVALUE_Struct fields)) (off + Z.of_N (sizeof_dtyp dt)) bytes) SUndef). *)
+    (*       cbn in H. *)
+    (*       forward H; auto. *)
+    (*     + rewrite lookup_all_index_length. *)
+    (*       reflexivity. *)
+    (*   - (* Packed structs *) *)
+    (*     rewrite sizeof_packed_struct_cons. *)
+
+    (*     inversion SUP. *)
+    (*     subst. *)
+    (*     rename H0 into FIELD_SUP. *)
+    (*     apply List.Forall_cons_iff in FIELD_SUP. *)
+    (*     destruct FIELD_SUP as [dt_SUP dts_SUP]. *)
+    (*     assert (is_supported (DTYPE_Packed_struct dts)) as SUP_STRUCT by (constructor; auto). *)
+
+    (*     cbn. *)
+    (*     rewrite lookup_all_index_append; [|apply sizeof_serialized; auto]. *)
+
+    (*     erewrite deserialize_packed_struct_element; auto. *)
+    (*     + erewrite <- sizeof_serialized; eauto. *)
+    (*       rewrite lookup_all_index_add_all_index_same_length; eauto. *)
+
+    (*       apply dvalue_serialized_not_sundef. *)
+    (*     + pose proof deserialize_sbytes_dvalue_all_not_sundef (DVALUE_Packed_struct fields) (DTYPE_Packed_struct dts) (lookup_all_index (off + Z.of_N (sizeof_dtyp dt)) (sizeof_dtyp (DTYPE_Packed_struct dts)) *)
+    (*                                                                                                                       (add_all_index (serialize_dvalue (DVALUE_Packed_struct fields)) (off + Z.of_N (sizeof_dtyp dt)) bytes) SUndef). *)
+    (*       cbn in H. *)
+    (*       forward H; auto. *)
+    (*     + rewrite lookup_all_index_length. *)
+    (*       reflexivity. *)
+    (*   - (* Arrays *) *)
+    (*     rename H into SZ. *)
+    (*     generalize dependent sz. *)
+    (*     generalize dependent xs. *)
+    (*     induction xs; *)
+    (*       intros IH IHdtyp sz SZ SUP. *)
+    (*     + cbn in *. *)
+    (*       subst. *)
+    (*       reflexivity. *)
+    (*     + cbn in SZ. *)
+    (*       subst. *)
+    (*       rewrite Nnat.Nat2N.inj_succ. *)
+    (*       cbn. *)
+
+    (*       assert (dvalue_has_dtyp a dt) as DTa. *)
+    (*       { *)
+    (*         apply IHdtyp. *)
+    (*         cbn. auto. *)
+    (*       } *)
+
+    (*       rewrite Nmult_Sn_m. *)
+    (*       rewrite lookup_all_index_append; [|apply sizeof_serialized; auto]. *)
+
+    (*       erewrite deserialize_array_element; auto. *)
+    (*       * inversion SUP; constructor; auto. *)
+    (*       * erewrite <- sizeof_serialized; eauto. *)
+    (*         rewrite lookup_all_index_add_all_index_same_length; eauto. *)
+
+    (*         apply dvalue_serialized_not_sundef. *)
+    (*       * (* Should be serialization of DVALUE_array xs *) *)
+    (*         replace (N.of_nat (Datatypes.length xs) * sizeof_dtyp dt)%N *)
+    (*           with (N.of_nat (N.to_nat (N.of_nat (Datatypes.length xs) * sizeof_dtyp dt))) by lia. *)
+    (*         rewrite lookup_all_index_add_all_index_same_length. *)
+
+    (*         apply all_not_sundef_fold_right_serialize. *)
+
+    (*         apply serialize_fold_length; intuition. *)
+    (*       * replace (sizeof_dtyp dt) with (N.of_nat (N.to_nat (sizeof_dtyp dt))) by lia. *)
+    (*         rewrite lookup_all_index_add_all_index_same_length. *)
+    (*         erewrite <- sizeof_serialized; intuition. *)
+    (*         lia. *)
+    (*         erewrite <- sizeof_serialized; intuition. *)
+    (*         lia. *)
+    (*       * rewrite IH; intuition. *)
+    (*         inversion SUP; auto. *)
+    (*       * cbn. *)
+
+    (*         unfold deserialize_sbytes. *)
+    (*         break_match. *)
+
+    (*         2: { *)
+    (*           assert (all_not_sundef *)
+    (*                     (lookup_all_index (off + Z.of_N (sizeof_dtyp dt)) *)
+    (*                                       (N.of_nat (Datatypes.length xs) * sizeof_dtyp dt) *)
+    (*                                       (add_all_index *)
+    (*                                          (fold_right (fun (dv : dvalue) (acc : list SByte) => serialize_dvalue dv ++ acc) [] *)
+    (*                                                      xs) (off + Z.of_N (sizeof_dtyp dt)) bytes) SUndef) = true) as CONTRA. *)
+    (*           replace (N.of_nat (Datatypes.length xs) * sizeof_dtyp dt)%N *)
+    (*             with (N.of_nat (N.to_nat (N.of_nat (Datatypes.length xs) * sizeof_dtyp dt))) by lia. *)
+    (*           rewrite lookup_all_index_add_all_index_same_length. *)
+
+    (*           apply all_not_sundef_fold_right_serialize. *)
+
+    (*           apply serialize_fold_length; intuition. *)
+
+    (*           rewrite Heqb in CONTRA. *)
+    (*           inversion CONTRA. *)
+    (*         } *)
+
+    (*         forward IHxs; intuition. *)
+    (*         forward IHxs; intuition. *)
+    (*         specialize (IHxs (Datatypes.length xs) eq_refl). *)
+    (*         forward IHxs. *)
+    (*         { inversion SUP; constructor; eauto. } *)
+
+    (*         cbn in IHxs. *)
+    (*         rewrite <- IHxs. *)
+
+    (*         rewrite all_not_sundef_deserialized; auto. *)
+    (*         erewrite <- sizeof_serialized. *)
+
+    (*         f_equal. *)
+
+    (*         repeat rewrite <- Nnat.Nat2N.inj_mul. *)
+    (*         rewrite lookup_all_index_add_all_index_same_length. *)
+    (*         rewrite lookup_all_index_add_all_index_same_length. *)
+    (*         reflexivity. *)
+
+    (*         { erewrite <- serialize_fold_length. *)
+    (*           erewrite <- sizeof_serialized. *)
+
+    (*           repeat rewrite <- Nnat.Nat2N.inj_mul. *)
+    (*           rewrite Nnat.Nat2N.id. *)
+    (*           reflexivity. *)
+
+    (*           eauto. *)
+    (*           intuition. *)
+    (*         } *)
+
+    (*         { erewrite <- serialize_fold_length. *)
+    (*           erewrite <- sizeof_serialized. *)
+
+    (*           repeat rewrite <- Nnat.Nat2N.inj_mul. *)
+    (*           rewrite Nnat.Nat2N.id. *)
+    (*           reflexivity. *)
+
+    (*           eauto. *)
+    (*           intuition. *)
+    (*         } *)
+
+    (*         eauto. *)
+    (*   - (* Vectors *) *)
+    (*     rename H into SZ. *)
+    (*     generalize dependent sz. *)
+    (*     generalize dependent xs. *)
+    (*     induction xs; *)
+    (*       intros IH IHdtyp sz SZ SUP. *)
+    (*     + cbn in *. *)
+    (*       subst. *)
+    (*       reflexivity. *)
+    (*     + cbn in SZ. *)
+    (*       subst. *)
+    (*       rewrite Nnat.Nat2N.inj_succ. *)
+    (*       cbn. *)
+
+    (*       assert (dvalue_has_dtyp a dt) as DTa. *)
+    (*       { *)
+    (*         apply IHdtyp. *)
+    (*         cbn. auto. *)
+    (*       } *)
+
+    (*       rewrite Nmult_Sn_m. *)
+    (*       rewrite lookup_all_index_append; [|apply sizeof_serialized; auto]. *)
+
+    (*       erewrite deserialize_vector_element; auto. *)
+    (*       * inversion SUP; constructor; auto. *)
+    (*       * erewrite <- sizeof_serialized; eauto. *)
+    (*         rewrite lookup_all_index_add_all_index_same_length; eauto. *)
+
+    (*         apply dvalue_serialized_not_sundef. *)
+    (*       * (* Should be serialization of DVALUE_vector xs *) *)
+    (*         replace (N.of_nat (Datatypes.length xs) * sizeof_dtyp dt)%N *)
+    (*           with (N.of_nat (N.to_nat (N.of_nat (Datatypes.length xs) * sizeof_dtyp dt))) by lia. *)
+    (*         rewrite lookup_all_index_add_all_index_same_length. *)
+
+    (*         apply all_not_sundef_fold_right_serialize. *)
+
+    (*         apply serialize_fold_length; intuition. *)
+    (*       * replace (sizeof_dtyp dt) with (N.of_nat (N.to_nat (sizeof_dtyp dt))) by lia. *)
+    (*         rewrite lookup_all_index_add_all_index_same_length. *)
+    (*         erewrite <- sizeof_serialized; intuition. *)
+    (*         lia. *)
+    (*         erewrite <- sizeof_serialized; intuition. *)
+    (*         lia. *)
+    (*       * rewrite IH; intuition. *)
+    (*         inversion SUP; subst; auto. *)
+    (*       * cbn. *)
+
+    (*         unfold deserialize_sbytes. *)
+    (*         break_match. *)
+
+    (*         2: { *)
+    (*           assert (all_not_sundef *)
+    (*                     (lookup_all_index (off + Z.of_N (sizeof_dtyp dt)) *)
+    (*                                       (N.of_nat (Datatypes.length xs) * sizeof_dtyp dt) *)
+    (*                                       (add_all_index *)
+    (*                                          (fold_right (fun (dv : dvalue) (acc : list SByte) => serialize_dvalue dv ++ acc) [] *)
+    (*                                                      xs) (off + Z.of_N (sizeof_dtyp dt)) bytes) SUndef) = true) as CONTRA. *)
+    (*           replace (N.of_nat (Datatypes.length xs) * sizeof_dtyp dt)%N *)
+    (*             with (N.of_nat (N.to_nat (N.of_nat (Datatypes.length xs) * sizeof_dtyp dt))) by lia. *)
+    (*           rewrite lookup_all_index_add_all_index_same_length. *)
+
+    (*           apply all_not_sundef_fold_right_serialize. *)
+
+    (*           apply serialize_fold_length; intuition. *)
+
+    (*           rewrite Heqb in CONTRA. *)
+    (*           inversion CONTRA. *)
+    (*         } *)
+
+    (*         forward IHxs; intuition. *)
+    (*         forward IHxs; intuition. *)
+    (*         specialize (IHxs (Datatypes.length xs) eq_refl). *)
+    (*         forward IHxs. *)
+    (*         { inversion SUP; constructor; eauto. } *)
+
+    (*         cbn in IHxs. *)
+    (*         rewrite <- IHxs. *)
+
+    (*         rewrite all_not_sundef_deserialized; auto. *)
+    (*         erewrite <- sizeof_serialized. *)
+
+    (*         f_equal. *)
+
+    (*         repeat rewrite <- Nnat.Nat2N.inj_mul. *)
+    (*         rewrite lookup_all_index_add_all_index_same_length. *)
+    (*         rewrite lookup_all_index_add_all_index_same_length. *)
+    (*         reflexivity. *)
+
+    (*         { erewrite <- serialize_fold_length. *)
+    (*           erewrite <- sizeof_serialized. *)
+
+    (*           repeat rewrite <- Nnat.Nat2N.inj_mul. *)
+    (*           rewrite Nnat.Nat2N.id. *)
+    (*           reflexivity. *)
+
+    (*           eauto. *)
+    (*           intuition. *)
+    (*         } *)
+
+    (*         { erewrite <- serialize_fold_length. *)
+    (*           erewrite <- sizeof_serialized. *)
+
+    (*           repeat rewrite <- Nnat.Nat2N.inj_mul. *)
+    (*           rewrite Nnat.Nat2N.id. *)
+    (*           reflexivity. *)
+
+    (*           eauto. *)
+    (*           intuition. *)
+    (*         } *)
+
+    (*         eauto. *)
+    (* Qed. *)
+
+    (* (** ** Write - Read *)
+    (*     The expected law: reading the key that has just been written to returns the written value. *)
+    (*     The only subtlety comes from the fact that it holds _if_ the read is performed at the type of *)
+    (*     the written value. *)
+    (*  *) *)
+    (* Lemma write_read : *)
+    (*   forall (m m' : memory_stack) (t : dtyp) (val : dvalue) (a : addr), *)
+    (*     is_supported t -> *)
+    (*     write m a val = inr m' -> *)
+    (*     dvalue_has_dtyp val t -> *)
+    (*     read m' a t = inr (dvalue_to_uvalue val). *)
+    (* Proof. *)
+    (*   unfold write, read; cbn. *)
+    (*   intros * SUP WR TYP. *)
+    (*   flatten_hyp WR; try inv_sum. *)
+    (*   destruct l,a as [id off]; inv_sum. *)
+    (*   rewrite get_logical_block_of_add_logical_block. *)
+    (*   cbn. *)
+    (*   unfold read_in_mem_block. *)
+    (*   rewrite deserialize_serialize; auto. *)
+    (* Qed. *)
+
+    (* Arguments add : simpl never. *)
+    (* Arguments lookup : simpl never. *)
+    (* Arguments logical_next_key : simpl never. *)
+
+    (* Lemma write_allocated : forall m a val m', *)
+    (*     write m a val = inr m' -> *)
+    (*     allocated a m. *)
+    (* Proof. *)
+    (*   unfold write; intros ((cm,lm),s) * WR; cbn in *. *)
+    (*   flatten_hyp WR; [| inv_sum]. *)
+    (*   destruct l,a; inv WR. *)
+    (*   cbn in *; eapply lookup_member; eauto. *)
+    (* Qed. *)
+
+    (* Lemma lookup_all_index_add_all_index_no_overlap : *)
+    (*   forall {A} bs off off' m (def : A) (sz : N), *)
+    (*     off' + Z.of_N sz <= off \/ off + (Z.of_nat (length bs)) <= off' -> *)
+    (*     lookup_all_index off' sz (add_all_index bs off m) def = *)
+    (*     lookup_all_index off' sz m def. *)
+    (* Proof. *)
+    (*   intros A; induction bs; intros off off' m def sz Hrange; auto. *)
+    (*   cbn. *)
+    (*   rewrite lookup_all_index_add_out; auto; try lia. *)
+    (*   apply IHbs; auto. *)
+    (*   destruct Hrange as [Hleft | Hright]; cbn in *; lia. *)
+    (*   destruct Hrange; cbn in *; lia. *)
+    (* Qed. *)
+
+    (* Lemma write_untouched: *)
+    (*   forall (m1 : memory_stack) (a : addr) (v : dvalue) (τ : dtyp) (m2 : memory_stack), *)
+    (*     dvalue_has_dtyp v τ -> *)
+    (*     write m1 a v = inr m2 -> *)
+    (*     forall (a' : addr) (τ' : dtyp), *)
+    (*       no_overlap_dtyp a τ a' τ' -> *)
+    (*       read m2 a' τ' = read m1 a' τ'. *)
+    (* Proof. *)
+    (*   intros ((cm,lm),s) [a off] v τ ((cm',lm'),s') TYP WR [a' off'] τ' INEQ. *)
+    (*   unfold read,write in *. *)
+    (*   cbn in *. *)
+    (*   flatten_hyp WR; try inv_sum. *)
+    (*   destruct l; inv_sum. *)
+    (*   apply no_overlap__not_overlaps in INEQ; *)
+    (*     unfold overlaps_dtyp, overlaps in INEQ; cbn in INEQ. *)
+    (*   unfold get_logical_block, get_logical_block_mem; cbn. *)
+    (*   destruct (Z.eq_dec a a') eqn:Haa'. *)
+    (*   - subst. rewrite lookup_add_eq. *)
+    (*     unfold get_logical_block,get_logical_block_mem in Heq. cbn in Heq. *)
+    (*     rewrite Heq. *)
+    (*     destruct (Z.le_gt_cases off (off' + (Z.of_N (sizeof_dtyp τ') - 1))) as [Hle | Hnle]. *)
+    (*     + destruct (Z.le_gt_cases off' (off + (Z.of_N (sizeof_dtyp τ) - 1))) as [Hle' | Hnle']. *)
+    (*       * exfalso. apply INEQ. lia. *)
+    (*       * (* Overlap because off + sizeof_dtyp τ < off', so second memory region is "to the right" *) *)
+    (*         unfold read_in_mem_block. *)
+    (*         rewrite lookup_all_index_add_all_index_no_overlap; auto. *)
+    (*         rewrite <- nat_N_Z. *)
+    (*         rewrite sizeof_serialized with (dt:=τ); auto; lia. *)
+    (*     + (* off' + sizeof_dtyp τ' < off, so second memory region is "to the left" *) *)
+    (*       unfold read_in_mem_block. *)
+    (*       rewrite lookup_all_index_add_all_index_no_overlap; auto. *)
+    (*       lia. *)
+    (*   - rewrite lookup_add_ineq; auto. *)
+    (* Qed. *)
+
+    Lemma write_succeeds : forall m1 v τ a aids,
+        uvalue_has_dtyp v τ ->
+        (* dtyp_fits m1 a τ -> *)
+        write_allowed (fst (ms_memory_stack m1)) (fst a) (snd a) (N.to_nat (sizeof_dtyp τ)) = inr aids ->
+        exists m2,
+          ErrSID_MemState_ms_runs_to (fun ms => write ms a v τ) m1 m2.
+    Proof.
+      intros m1 v τ a aids TYP CAN.
+      (* destruct CAN as (sz & bytes & cid & BLOCK & SIZE). *)
+
+      exists m1. (* (mkMemState (add_all_index mem) (ms_sid m1) (ms_prov m1)). *)
+      unfold ErrSID_MemState_ms_runs_to.
+
+      unfold write.
+      unfold write_memory.
+      unfold write_allowed_errsid.
+
+      destruct m1.
+
+      destruct ms_memory_stack0.
+      change (ms_memory_stack {| ms_memory_stack := (m, f); ms_sid := ms_sid0; ms_prov := ms_prov0 |}) with (m, f).
+
+      break_match; subst.
+      break_match; subst.
+
+      cbn in CAN.
+      rewrite CAN.
+
+      cbn.
+    Admitted.
+
+    (* Lemma read_write_succeeds : *)
+    (*   forall m ptr τ val v, *)
+    (*     read m ptr τ = inr val -> *)
+    (*     dvalue_has_dtyp v τ -> *)
+    (*     exists m2, write m ptr v = inr m2. *)
+    (* Proof. *)
+    (*   intros m ptr τ val v READ TYP. *)
+    (*   unfold read in *. *)
+    (*   destruct (get_logical_block m (fst ptr)) eqn:LBLOCK; inversion READ. *)
+    (*   clear H0. *)
+
+    (*   destruct l as [sz bytes cid]. *)
+    (*   exists (add_logical_block (fst ptr) (LBlock sz (add_all_index (serialize_dvalue v) (snd ptr) bytes) cid) m). *)
+    (*   unfold write. *)
+    (*   rewrite LBLOCK. *)
+    (*   cbn. destruct ptr. reflexivity. *)
+    (* Qed. *)
+
+    (* Lemma write_correct : forall m1 a v m2, *)
+    (*     write m1 a v = inr m2 -> *)
+    (*     write_spec m1 a v m2. *)
+    (* Proof. *)
+    (*   intros; split; [| split]; eauto using write_allocated, write_read, write_untouched. *)
+    (* Qed. *)
+
+    (* Lemma write_block_preserves : *)
+    (*   forall m1 m2 (a a' : addr) v sz bytes cid, *)
+    (*     write m1 a v = inr m2 -> *)
+    (*     get_logical_block m1 (fst a') = Some (LBlock sz bytes cid) -> *)
+    (*     exists bytes', get_logical_block m2 (fst a') = Some (LBlock sz bytes' cid). *)
+    (* Proof. *)
+    (*   intros m1 m2 a a' v sz bytes cid WRITE GET. *)
+    (*   destruct m1, m2; cbn in *. *)
+    (*   unfold write in WRITE. *)
+    (*   cbn in WRITE. *)
+    (*   break_match_hyp; inv WRITE. *)
+    (*   destruct l. *)
+    (*   destruct a, a'. cbn in *. *)
+    (*   inv H0. *)
+
+    (*   destruct (Z.eq_dec z z1) as [EQ | NEQ]. *)
+    (*   - subst. *)
+    (*     rewrite GET in Heqo. inv Heqo. *)
+    (*     rewrite get_logical_block_of_add_logical_block_mem. *)
+    (*     eexists. *)
+    (*     reflexivity. *)
+    (*   - exists bytes. *)
+    (*     erewrite get_logical_block_of_add_logical_block_mem_neq; eauto. *)
+    (* Qed. *)
+
+    (* Lemma dtyp_fits_after_write : *)
+    (*   forall m m' ptr ptr' τ τ', *)
+    (*     dtyp_fits m ptr τ -> *)
+    (*     write m ptr' τ' = inr m' -> *)
+    (*     dtyp_fits m' ptr τ. *)
+    (* Proof. *)
+    (*   intros m m' ptr ptr' τ τ' FITS WRITE. *)
+    (*   unfold dtyp_fits in *. *)
+    (*   destruct FITS as (sz & bytes & cid & GET & BOUNDS). *)
+    (*   eapply write_block_preserves in WRITE; eauto. destruct WRITE as (bytes' & WRITE). *)
+    (*   exists sz. exists bytes'. exists cid. *)
+    (*   split; eauto. *)
+    (* Qed. *)
+
+    (* Lemma read_in_mem_block_write_to_mem_block : *)
+    (*   forall bytes offset val τ, *)
+    (*     is_supported τ -> *)
+    (*     dvalue_has_dtyp val τ -> *)
+    (*     read_in_mem_block (write_to_mem_block bytes offset val) offset τ = dvalue_to_uvalue val. *)
+    (* Proof. *)
+    (*   intros bytes offset val τ SUP H. *)
+    (*   unfold read_in_mem_block, write_to_mem_block. *)
+    (*   rewrite deserialize_serialize; eauto. *)
+    (* Qed. *)
+
+    (* Lemma write_array_cell_get_array_cell : *)
+    (*   forall (m m' : memory_stack) (t : dtyp) (val : dvalue) (a : addr) (i : nat), *)
+    (*     write_array_cell m a i t val = inr m' -> *)
+    (*     is_supported t -> *)
+    (*     dvalue_has_dtyp val t -> *)
+    (*     get_array_cell m' a i t = inr (dvalue_to_uvalue val). *)
+    (* Proof. *)
+    (*   intros m m' t val a i WRITE SUP TYP. *)
+    (*   destruct a; cbn in *. *)
+    (*   break_match_hyp; inv WRITE. *)
+    (*   destruct l. *)
+    (*   inversion H0; subst. *)
+    (*   rewrite get_logical_block_of_add_logical_block. *)
+    (*   rewrite read_in_mem_block_write_to_mem_block; eauto. *)
+    (* Qed. *)
+
+    (* (* TODO: make this more general? I.e. write / read different types? *) *)
+    (* Lemma read_in_mem_block_write_to_mem_block_untouched : *)
+    (*   forall offset offset' bytes val τ, *)
+    (*     dvalue_has_dtyp val τ -> *)
+    (*     offset' + Z.of_N (sizeof_dtyp τ) <= offset \/ offset + Z.of_N (sizeof_dtyp τ) <= offset' -> *)
+    (*     read_in_mem_block (write_to_mem_block bytes offset val) offset' τ = read_in_mem_block bytes offset' τ. *)
+    (* Proof. *)
+    (*   intros offset offset' bytes val τ TYP OUT. *)
+    (*   unfold read_in_mem_block, write_to_mem_block. *)
+    (*   rewrite lookup_all_index_add_all_index_no_overlap; eauto. *)
+    (*   destruct OUT. *)
+    (*   - left. auto. *)
+    (*   - right. rewrite <- nat_N_Z. erewrite sizeof_serialized; eauto. *)
+    (* Qed. *)
+
+    (* Lemma write_array_cell_untouched : *)
+    (*   forall (m m' : memory_stack) (t : dtyp) (val : dvalue) (a : addr) (i : nat) (i' : nat), *)
+    (*     write_array_cell m a i t val = inr m' -> *)
+    (*     dvalue_has_dtyp val t -> *)
+    (*     DynamicValues.Int64.unsigned (DynamicValues.Int64.repr (Z.of_nat i)) <> DynamicValues.Int64.unsigned (DynamicValues.Int64.repr (Z.of_nat i')) -> *)
+    (*     get_array_cell m' a i' t = get_array_cell m a i' t. *)
+    (* Proof. *)
+    (*   intros m m' t val a i i' WRITE TYP NEQ. *)
+    (*   destruct a; cbn in *. *)
+    (*   break_match_hyp; inv WRITE. *)
+    (*   destruct l. *)
+    (*   inversion H0; subst. *)
+    (*   rewrite get_logical_block_of_add_logical_block. *)
+    (*   rewrite read_in_mem_block_write_to_mem_block_untouched; eauto. *)
+
+    (*   destruct (Z_lt_ge_dec (DynamicValues.Int64.unsigned (DynamicValues.Int64.repr (Z.of_nat i'))) (DynamicValues.Int64.unsigned (DynamicValues.Int64.repr (Z.of_nat i)))) as [LT | GE]. *)
+    (*   - left. *)
+    (*     rewrite <- Z.add_assoc. *)
+    (*     apply Z.add_le_mono_l. *)
+    (*     replace (DynamicValues.Int64.unsigned (DynamicValues.Int64.repr (Z.of_nat i')) * Z.of_N (sizeof_dtyp t) + Z.of_N (sizeof_dtyp t)) with ((1 + DynamicValues.Int64.unsigned (DynamicValues.Int64.repr (Z.of_nat i'))) * Z.of_N (sizeof_dtyp t)) by lia. *)
+    (*     apply Zmult_le_compat_r; eauto; lia. *)
+    (*   - right. *)
+    (*     rewrite <- Z.add_assoc. *)
+    (*     apply Z.add_le_mono_l. *)
+
+    (*     (* if i <> i' then the conversions shouldn't overlap either *) *)
+    (*     assert (DynamicValues.Int64.unsigned (DynamicValues.Int64.repr (Z.of_nat i')) > *)
+    (*             DynamicValues.Int64.unsigned (DynamicValues.Int64.repr (Z.of_nat i))) by lia. *)
+
+    (*     replace (DynamicValues.Int64.unsigned (DynamicValues.Int64.repr (Z.of_nat i)) * Z.of_N (sizeof_dtyp t) + Z.of_N (sizeof_dtyp t)) with ((1 + DynamicValues.Int64.unsigned (DynamicValues.Int64.repr (Z.of_nat i))) * Z.of_N (sizeof_dtyp t)) by lia. *)
+    (*     apply Zmult_le_compat_r; eauto; lia. *)
+    (* Qed. *)
+
+    (* Lemma write_array_cell_untouched_ptr_block : *)
+    (*   forall (m m' : memory_stack) (t : dtyp) (val : dvalue) (a a' : addr) (i i' : nat), *)
+    (*     write_array_cell m a i t val = inr m' -> *)
+    (*     dvalue_has_dtyp val t -> *)
+    (*     fst a' <> fst a -> *)
+    (*     get_array_cell m' a' i' t = get_array_cell m a' i' t. *)
+    (* Proof. *)
+    (*   intros m m' t val a a' i i' WRITE TYP BLOCK_NEQ. *)
+    (*   destruct a as [b1 o1]. *)
+    (*   destruct a' as [b2 o2]. *)
+    (*   unfold get_array_cell. *)
+    (*   cbn in WRITE. *)
+    (*   break_match_hyp; inv WRITE. *)
+    (*   destruct l. *)
+    (*   inv H0. *)
+    (*   rewrite get_logical_block_of_add_logical_block_neq; eauto. *)
+    (* Qed. *)
+
+    (* Lemma lookup_mapsto : *)
+    (*   forall {A} k m (v : A), *)
+    (*     lookup k m = Some v <-> IM.MapsTo k v m. *)
+    (* Proof. *)
+    (*   intros A k m v. *)
+    (*   split. *)
+    (*   - apply IM.find_2. *)
+    (*   - apply IM.find_1. *)
+    (* Qed. *)
+
+    (* Lemma all_neq_not_in: *)
+    (*   forall {A} (m : A) l, *)
+    (*     Forall (fun a => a <> m) l -> ~ In m l. *)
+    (* Proof. *)
+    (*   intros A m l ALL. *)
+    (*   induction ALL; intros IN; inversion IN. *)
+    (*   - subst; contradiction. *)
+    (*   - contradiction. *)
+    (* Qed. *)
+
+    (* Lemma assoc_list_in_key_in : *)
+    (*   forall A k v l, *)
+    (*     SetoidList.InA (IM.eq_key_elt (elt:=A)) (k, v) l -> *)
+    (*     In k (map fst l). *)
+    (* Proof. *)
+    (*   intros A k v l IN. *)
+    (*   induction IN as [[k' v'] l EQ | [k' v'] l INA IH]. *)
+    (*   - cbn. cbv in EQ. intuition. *)
+    (*   - cbn. auto. *)
+    (* Qed. *)
+
+    (* Lemma no_key_not_in : *)
+    (*   forall A l k v, *)
+    (*     (forall a : Z, In a (map fst l) -> a <> k) -> *)
+    (*     ~ SetoidList.InA (IM.eq_key_elt (elt:=A)) (k, v) l. *)
+    (* Proof. *)
+    (*   intros A l k v NOKEY. *)
+    (*   intros IN. apply assoc_list_in_key_in in IN. *)
+    (*   specialize (NOKEY k IN). *)
+    (*   contradiction. *)
+    (* Qed. *)
+
+    (* Lemma next_logical_key_fresh : forall lm, *)
+    (*     ~ member (logical_next_key lm) lm. *)
+    (* Proof. *)
+    (*   intros lm MEM. *)
+    (*   unfold logical_next_key in MEM. *)
+    (*   apply member_lookup in MEM as [lb LUP]. *)
+    (*   apply lookup_mapsto in LUP. *)
+    (*   apply IM.elements_1 in LUP. *)
+    (*   assert (forall a : Z, In a (map fst (IM.elements (elt:=logical_block) lm)) -> a <> 1 + maximumBy Z.leb (-1) (map fst (IM.elements (elt:=logical_block) lm))) as NOKEY. *)
+    (*   - intros a IN. *)
+    (*     apply (maximumBy_Z_correct (-1)) in IN. *)
+    (*     apply Zle_bool_imp_le in IN. *)
+    (*     lia. *)
+    (*   - apply no_key_not_in with (v:=lb) in NOKEY. *)
+    (*     contradiction. *)
+    (* Qed. *)
+
+    (* Lemma lookup_init_block_undef : *)
+    (*   forall n, *)
+    (*     lookup 0 (init_block_undef n empty) = Some SUndef. *)
+    (* Proof. *)
+    (*   induction n; auto. *)
+    (*   cbn. *)
+    (*   rewrite lookup_add_ineq; [|lia]. *)
+    (*   auto. *)
+    (* Qed. *)
+
+    (* Lemma lookup_init_block : *)
+    (*   forall n, *)
+    (*     (n > 0)%N -> *)
+    (*     lookup 0 (init_block n) = Some SUndef. *)
+    (* Proof. *)
+    (*   intros n SZ. *)
+    (*   pose proof Nnat.N2Nat.id n. *)
+    (*   induction (N.of_nat (N.to_nat n)); [lia|]. *)
+    (*   subst. *)
+    (*   cbn. *)
+    (*   apply lookup_init_block_undef. *)
+    (* Qed. *)
+
+    (* Lemma all_not_sundef_init : *)
+    (*   forall n, *)
+    (*     (n > 0)%N -> *)
+    (*     all_not_sundef (lookup_all_index 0 n (init_block n) SUndef) = false. *)
+    (* Proof. *)
+    (*   destruct n; intros SZ. *)
+    (*   inv SZ. *)
+    (*   cbn. *)
+
+    (*   pose proof Pos2Nat.is_succ p as [n PN]. *)
+    (*   rewrite PN. *)
+    (*   cbn. *)
+
+    (*   rewrite lookup_init_block_undef. *)
+    (*   reflexivity. *)
+    (* Qed. *)
+
+    (* (* This is false for VOID, and 0 length arrays *) *)
+    (* Lemma read_empty_block : forall τ, *)
+    (*     (sizeof_dtyp τ > 0)%N -> *)
+    (*     read_in_mem_block (make_empty_mem_block τ) 0 τ = UVALUE_Undef τ. *)
+    (* Proof. *)
+    (*   unfold read_in_mem_block. *)
+    (*   unfold make_empty_mem_block. *)
+    (*   unfold deserialize_sbytes. *)
+    (*   intros τ. induction τ; intros SZ; try solve [reflexivity | cbn in SZ; inv SZ | rewrite all_not_sundef_init; auto]. *)
+    (* Qed. *)
+
+    (* (* TODO: finish a less specialized version of this *) *)
+    (* Lemma read_array_not_pointer : forall mem a τ sz v dv, *)
+    (*     not_undef v -> *)
+    (*     read mem a (DTYPE_Array sz τ) = inr v -> *)
+    (*     uvalue_to_dvalue v = inr dv -> *)
+    (*     ~ dvalue_has_dtyp dv DTYPE_Pointer. *)
+    (* Proof. *)
+    (*   intros mem a τ sz v dv NU READ CONVERT. *)
+    (*   intros TYP. *)
+    (*   inversion TYP. *)
+    (*   subst. *)
+    (*   unfold read in READ. *)
+    (*   break_match; try discriminate READ. *)
+    (*   break_match; subst. *)
+    (*   unfold read_in_mem_block in READ. *)
+    (*   unfold deserialize_sbytes in READ. *)
+    (*   break_match. *)
+    (*   - (* Fully defined *) *)
+    (*     inversion READ; subst. *)
+    (*     cbn in CONVERT. *)
+    (*     break_match; inversion CONVERT. *)
+    (*   - (* Undefined *) *)
+    (*     inversion READ; subst; *)
+    (*       eapply NU; eauto. *)
+    (* Qed. *)
+
+    (* Lemma allocate_succeeds : forall m1 τ, *)
+    (*     non_void τ -> *)
+    (*     exists m2 a, allocate m1 τ = inr (m2, a). *)
+    (* Proof. *)
+    (*   intros m1 τ NV. *)
+    (*   destruct m1 as [m fs]. *)
+    (*   destruct fs as [|f fs]. *)
+    (*   - destruct τ eqn:Hτ; cbn; repeat rewrite <- Hτ; *)
+    (*       exists (add_logical_block_mem (next_logical_key (m, Singleton f)) (make_empty_logical_block τ) m, *)
+    (*               Singleton (next_logical_key (m, Singleton f) :: f)); *)
+    (*       exists (next_logical_key (m, Singleton f), 0); *)
+    (*       auto; exfalso; auto. *)
+    (*   - destruct τ eqn:Hτ; cbn; repeat rewrite <- Hτ; *)
+    (*       exists (add_logical_block_mem (next_logical_key (m, Snoc f fs)) (make_empty_logical_block τ) m, *)
+    (*               Snoc f (next_logical_key (m, Snoc f fs) :: fs)); *)
+    (*       exists (next_logical_key (m, Snoc f fs), 0); *)
+    (*       auto; exfalso; auto. *)
+    (* Qed. *)
+
+    (* Lemma allocate_non_void : forall m τ x, *)
+    (*     allocate m τ = inr x -> *)
+    (*     non_void τ. *)
+    (* Proof. *)
+    (*   intros m τ x H. *)
+    (*   destruct τ; inversion H; intros NV; inversion NV. *)
+    (* Qed. *)
+
+    (* Lemma allocate_correct : forall m1 τ m2 a, *)
+    (*     allocate m1 τ = inr (m2,a) -> *)
+    (*     allocate_spec m1 τ m2 a. *)
+    (* Proof. *)
+    (*   intros ((cm,lm),s) * EQ; *)
+    (*     destruct s as [|f s]; apply allocate_inv in EQ as [NV [EQm2 EQa]]; subst; cbn. *)
+    (*   - split. *)
+    (*     + cbn. apply next_logical_key_fresh. *)
+    (*     + { split. *)
+    (*         + intros SIZE. *)
+    (*           unfold read; cbn. *)
+    (*           unfold get_logical_block, get_logical_block_mem; cbn. *)
+    (*           rewrite lookup_add_eq; cbn. *)
+    (*           unfold non_void in NV. *)
+    (*           f_equal; apply read_empty_block. *)
+    (*           lia. *)
+    (*         + intros * ALLOC NOVER. *)
+    (*           unfold read; cbn. *)
+    (*           unfold get_logical_block, get_logical_block_mem; cbn. *)
+
+    (*           cbn in ALLOC. *)
+
+    (*           apply no_overlap__not_overlaps in NOVER. *)
+    (*           unfold next_logical_key, next_logical_key_mem, overlaps in *. *)
+    (*           cbn in *. *)
+    (*           destruct (Z.eq_dec (logical_next_key lm) (fst a')) as [Ha' | Ha']. *)
+    (*           -- (* Bogus branch where a' is the freshly allocated block *) *)
+    (*             exfalso. eapply next_logical_key_fresh; erewrite Ha'; eauto. *)
+    (*           -- (* Good branch *) *)
+    (*             rewrite lookup_add_ineq; auto. *)
+    (*       } *)
+    (*   - split. *)
+    (*     + cbn. apply next_logical_key_fresh. *)
+    (*     + { split. *)
+    (*         + intros SIZE. *)
+    (*           unfold read; cbn. *)
+    (*           unfold get_logical_block, get_logical_block_mem; cbn. *)
+    (*           rewrite lookup_add_eq; cbn. *)
+    (*           f_equal; apply read_empty_block. *)
+    (*           lia. *)
+    (*         + intros * ALLOC NOVER. *)
+    (*           unfold read; cbn. *)
+    (*           unfold get_logical_block, get_logical_block_mem; cbn. *)
+
+    (*           cbn in ALLOC. *)
+
+    (*           apply no_overlap__not_overlaps in NOVER. *)
+    (*           unfold next_logical_key, next_logical_key_mem, overlaps in *. *)
+    (*           cbn in *. *)
+    (*           destruct (Z.eq_dec (logical_next_key lm) (fst a')) as [Ha' | Ha']. *)
+    (*           -- (* Bogus branch where a' is the freshly allocated block *) *)
+    (*             exfalso. eapply next_logical_key_fresh; erewrite Ha'; eauto. *)
+    (*           -- (* Good branch *) *)
+    (*             rewrite lookup_add_ineq; auto. *)
+    (*       } *)
+    (* Qed. *)
+
+    (* Lemma allocated_get_logical_block : *)
+    (*   forall a m, *)
+    (*     allocated a m -> *)
+    (*     exists b, get_logical_block m (fst a) = Some b. *)
+    (* Proof. *)
+    (*   intros a m H. *)
+    (*   unfold allocated in H. *)
+    (*   destruct m as [[cm lm] fs]. *)
+    (*   apply member_lookup in H as [b LUP]. *)
+    (*   exists b. unfold get_logical_block. cbn. *)
+    (*   unfold get_logical_block_mem. cbn. *)
+    (*   auto. *)
+    (* Qed. *)
+
+    (* Lemma read_array: forall m size τ i a elem_addr, *)
+    (*     allocated a m -> *)
+    (*     handle_gep_addr (DTYPE_Array size τ) a [DVALUE_I64 (repr 0); DVALUE_I64 (repr (Z.of_nat i))] = inr elem_addr -> *)
+    (*     read m elem_addr τ = get_array_cell m a i τ. *)
+    (* Proof. *)
+    (*   intros m size τ i a elem_addr ALLOC GEP. *)
+    (*   unfold get_array_cell. *)
+    (*   destruct a. *)
+    (*   unfold read. *)
+    (*   cbn in GEP. *)
+    (*   inversion GEP. subst. *)
+    (*   cbn. *)
+    (*   destruct (get_logical_block m z) eqn:GET. *)
+    (*   - destruct l. *)
+    (*     cbn. *)
+    (*     rewrite Int64.unsigned_repr. *)
+    (*     + replace (z0 + Z.of_N (size * sizeof_dtyp τ) * 0 + *)
+    (*                DynamicValues.Int64.unsigned (DynamicValues.Int64.repr (Z.of_nat i)) * Z.of_N (sizeof_dtyp τ)) *)
+    (*         with  (z0 + DynamicValues.Int64.unsigned (DynamicValues.Int64.repr (Z.of_nat i)) * Z.of_N (sizeof_dtyp τ)) *)
+    (*         by lia. *)
+    (*       reflexivity. *)
+    (*     + unfold Int64.max_unsigned. cbn. lia. *)
+    (*   - pose proof allocated_get_logical_block (z, z0) m ALLOC as [b GETSOME]. *)
+    (*     cbn in GETSOME. *)
+    (*     rewrite GET in GETSOME. *)
+    (*     inversion GETSOME. *)
+    (* Qed. *)
+
+    (* Lemma can_read_allocated : *)
+    (*   forall ptr τ v m, *)
+    (*     read m ptr τ = inr v -> *)
+    (*     allocated ptr m. *)
+    (* Proof. *)
+    (*   intros ptr τ v m READ. *)
+    (*   unfold read in READ. *)
+    (*   destruct (get_logical_block m (fst ptr)) eqn:LBLOCK. *)
+    (*   - destruct l. *)
+    (*     red. unfold get_logical_block, get_logical_block_mem in LBLOCK. *)
+    (*     apply lookup_member in LBLOCK. *)
+    (*     do 2 destruct m. *)
+    (*     cbn in LBLOCK. *)
+    (*     auto. *)
+    (*   - inversion READ. *)
+    (* Qed. *)
+
+    (* Lemma allocated_can_read : *)
+    (*   forall a m τ, *)
+    (*     allocated a m -> *)
+    (*     exists v, read m a τ = inr v. *)
+    (* Proof. *)
+    (*   intros a [[cm lm] fs] τ ALLOC. *)
+    (*   apply allocated_get_logical_block in ALLOC. *)
+    (*   destruct ALLOC as [b GET]. *)
+    (*   unfold read. *)
+    (*   rewrite GET. *)
+    (*   destruct b. *)
+    (*   cbn. *)
+    (*   exists (read_in_mem_block bytes (snd a) τ). reflexivity. *)
+    (* Qed. *)
+
+    (* Lemma freshly_allocated_different_blocks : *)
+    (*   forall ptr1 ptr2 τ m1 m2, *)
+    (*     allocate m1 τ = inr (m2, ptr2) -> *)
+    (*     allocated ptr1 m1 -> *)
+    (*     fst ptr2 <> fst ptr1. *)
+    (* Proof. *)
+    (*   intros ptr1 ptr2 τ m1 m2 ALLOC INM1 EQ. *)
+    (*   pose proof (allocate_correct ALLOC) as (ALLOC_FRESH & ALLOC_NEW & ALLOC_OLD). *)
+    (*   apply ALLOC_FRESH. *)
+    (*   unfold allocated in *. *)
+    (*   destruct m1 as [[cm1 lm1] fs1]. *)
+    (*   rewrite EQ. *)
+    (*   auto. *)
+    (* Qed. *)
+
+    (* Lemma freshly_allocated_no_overlap_dtyp : *)
+    (*   forall ptr1 ptr2 τ τ' m1 m2, *)
+    (*     allocate m1 τ' = inr (m2, ptr2) -> *)
+    (*     allocated ptr1 m1 -> *)
+    (*     no_overlap_dtyp ptr2 τ' ptr1 τ. *)
+    (* Proof. *)
+    (*   intros ptr1 ptr2 τ τ' m1 m2 ALLOC INM1. *)
+    (*   repeat red. *)
+    (*   left. *)
+    (*   eapply freshly_allocated_different_blocks; eauto. *)
+    (* Qed. *)
+
+    (* Lemma no_overlap_dtyp_different_blocks : *)
+    (*   forall a b τ τ', *)
+    (*     fst a <> fst b -> *)
+    (*     no_overlap_dtyp a τ b τ'. *)
+    (* Proof. *)
+    (*   intros a b τ τ' H. *)
+    (*   unfold no_overlap_dtyp, no_overlap. *)
+    (*   auto. *)
+    (* Qed. *)
+
+    (* Lemma read_array_exists : forall m size τ i a, *)
+    (*     allocated a m -> *)
+    (*     exists elem_addr, *)
+    (*       handle_gep_addr (DTYPE_Array size τ) a [DVALUE_I64 (repr 0); DVALUE_I64 (repr (Z.of_nat i))] = inr elem_addr /\ read m elem_addr τ = get_array_cell m a i τ. *)
+    (* Proof. *)
+    (*   intros m size τ i a ALLOC. *)
+    (*   destruct a. *)
+    (*   exists (z, *)
+    (*           z0 + Z.of_N size * Z.of_N (sizeof_dtyp τ) * DynamicValues.Int64.unsigned (DynamicValues.Int64.repr 0) + *)
+    (*           DynamicValues.Int64.unsigned (DynamicValues.Int64.repr (Z.of_nat i)) * Z.of_N (sizeof_dtyp τ)). *)
+    (*   split. *)
+    (*   - cbn. *)
+    (*     rewrite Int64.unsigned_repr. *)
+    (*     replace (z0 + Z.of_N (size * sizeof_dtyp τ) * 0 + *)
+    (*              DynamicValues.Int64.unsigned (DynamicValues.Int64.repr (Z.of_nat i)) * Z.of_N (sizeof_dtyp τ)) *)
+    (*       with (z0 + DynamicValues.Int64.unsigned (DynamicValues.Int64.repr (Z.of_nat i)) * Z.of_N (sizeof_dtyp τ)) *)
+    (*       by lia. *)
+    (*     replace (z0 + Z.of_N size * Z.of_N (sizeof_dtyp τ) * 0 + *)
+    (*              Int64.unsigned (Int64.repr (Z.of_nat i)) * Z.of_N (sizeof_dtyp τ)) *)
+    (*       with (z0 + DynamicValues.Int64.unsigned (DynamicValues.Int64.repr (Z.of_nat i)) * Z.of_N (sizeof_dtyp τ)) by lia. *)
+    (*     reflexivity. *)
+    (*     unfold Int64.max_unsigned. cbn. lia. *)
+    (*   - eapply read_array; cbn; eauto. *)
+    (*     rewrite N2Z.inj_mul. *)
+    (*     reflexivity. *)
+    (* Qed. *)
+
+    (* Lemma write_array_lemma : forall m size τ i a elem_addr v, *)
+    (*     allocated a m -> *)
+    (*     handle_gep_addr (DTYPE_Array size τ) a [DVALUE_I64 (repr 0); DVALUE_I64 (repr (Z.of_nat i))] = inr elem_addr -> *)
+    (*     write m elem_addr v = write_array_cell m a i τ v. *)
+    (* Proof. *)
+    (*   intros m size τ i a elem_addr v ALLOC GEP. *)
+    (*   unfold write_array_cell. *)
+    (*   destruct a. *)
+    (*   unfold write. *)
+    (*   cbn in GEP. *)
+    (*   inversion GEP. subst. *)
+    (*   cbn. *)
+    (*   destruct (get_logical_block m z) eqn:GET. *)
+    (*   - destruct l. *)
+    (*     cbn. *)
+    (*     rewrite Int64.unsigned_repr. *)
+    (*     + replace (z0 + Z.of_N (size * sizeof_dtyp τ) * 0 + *)
+    (*                DynamicValues.Int64.unsigned (DynamicValues.Int64.repr (Z.of_nat i)) * Z.of_N (sizeof_dtyp τ)) *)
+    (*         with  (z0 + DynamicValues.Int64.unsigned (DynamicValues.Int64.repr (Z.of_nat i)) * Z.of_N (sizeof_dtyp τ)) *)
+    (*         by lia. *)
+
+    (*       reflexivity. *)
+    (*     + unfold Int64.max_unsigned. cbn. lia. *)
+    (*   - pose proof allocated_get_logical_block (z, z0) m ALLOC as [b GETSOME]. *)
+    (*     cbn in GETSOME. *)
+    (*     rewrite GET in GETSOME. *)
+    (*     inversion GETSOME. *)
+    (* Qed. *)
+
+    (* Lemma write_array_exists : forall m size τ i a v, *)
+    (*     allocated a m -> *)
+    (*     exists elem_addr, *)
+    (*       handle_gep_addr (DTYPE_Array size τ) a [DVALUE_I64 (repr 0); DVALUE_I64 (repr (Z.of_nat i))] = inr elem_addr /\ write m elem_addr v = write_array_cell m a i τ v. *)
+    (* Proof. *)
+    (*   intros m size τ i a v ALLOC. *)
+    (*   destruct a. *)
+    (*   exists (z, *)
+    (*           z0 + Z.of_N (size * sizeof_dtyp τ) * DynamicValues.Int64.unsigned (DynamicValues.Int64.repr 0) + *)
+    (*           DynamicValues.Int64.unsigned (DynamicValues.Int64.repr (Z.of_nat i)) * Z.of_N (sizeof_dtyp τ)). *)
+    (*   split. *)
+    (*   - cbn. *)
+    (*     rewrite Int64.unsigned_repr. *)
+    (*     replace (z0 + Z.of_N (size * sizeof_dtyp τ) * 0 + *)
+    (*              DynamicValues.Int64.unsigned (DynamicValues.Int64.repr (Z.of_nat i)) * Z.of_N (sizeof_dtyp τ)) *)
+    (*       with  (z0 + DynamicValues.Int64.unsigned (DynamicValues.Int64.repr (Z.of_nat i)) * Z.of_N (sizeof_dtyp τ)) *)
+    (*       by lia. *)
+    (*     reflexivity. *)
+    (*     unfold Int64.max_unsigned. cbn. lia. *)
+    (*   - eapply write_array_lemma; cbn; eauto. *)
+    (* Qed. *)
+
+    (* Lemma write_preserves_allocated : *)
+    (*   forall {m1 m2 ptr ptr' v}, *)
+    (*     allocated ptr' m1 -> *)
+    (*     write m1 ptr v = inr m2 -> *)
+    (*     allocated ptr' m2. *)
+    (* Proof. *)
+    (*   intros m1 m2 ptr ptr' v ALLOC WRITE. *)
+    (*   unfold allocated in *. *)
+    (*   destruct m1 as [[cm1 lm1] f1]. *)
+    (*   destruct m2 as [[cm2 lm2] f2]. *)
+
+    (*   unfold write in WRITE. *)
+    (*   destruct (get_logical_block (cm1, lm1, f1) (fst ptr)) eqn:LB. *)
+    (*   - setoid_rewrite LB in WRITE. *)
+    (*     destruct l. *)
+    (*     destruct ptr as [ptr_b ptr_i]. *)
+    (*     inversion WRITE; subst. *)
+    (*     destruct ptr' as [ptr'_b ptr'_i]. *)
+    (*     eapply member_add_preserved; auto. *)
+    (*   - setoid_rewrite LB in WRITE. *)
+    (*     inversion WRITE. *)
+    (* Qed. *)
+
+    (* Lemma dtyp_fits_allocated : *)
+    (*   forall m a τ, *)
+    (*     dtyp_fits m a τ -> *)
+    (*     allocated a m. *)
+    (* Proof. *)
+    (*   intros m a τ FITS. *)
+    (*   unfold allocated. *)
+
+    (*   unfold dtyp_fits in FITS. *)
+    (*   destruct FITS as (sz & bytes & cid & LB & SIZE). *)
+
+    (*   (* TODO: Make this part of the allocated / get_logical_block lemma *) *)
+    (*   unfold get_logical_block, get_logical_block_mem in LB. *)
+    (*   destruct m as [[cm lm] f]. *)
+    (*   cbn in LB. *)
+    (*   eapply lookup_member; eauto. *)
+    (* Qed. *)
+
+    (* Lemma NM_NS_In {elt:Type} (k:IM.key) (m:IM.t elt): *)
+    (*   IM.In k m -> *)
+    (*   IS.In k (ISP.of_list (map fst (IM.elements  m))). *)
+    (* Proof. *)
+    (*   pose proof (IM.elements_3w m) as U. *)
+    (*   intros H. *)
+    (*   rewrite <- IP.of_list_3 with (s:=m) in H. *)
+    (*   unfold IP.of_list, IP.to_list in H. *)
+    (*   generalize dependent (IM.elements m). intros l U H. *)
+    (*   induction l. *)
+    (*   - *)
+    (*     simpl in H. *)
+    (*     apply IP.F.empty_in_iff in H. *)
+    (*     tauto. *)
+    (*   - *)
+    (*     destruct a as [k' v]. *)
+    (*     simpl in *. *)
+    (*     destruct (Z.eq_decidable k k') as [K|NK]. *)
+    (*     + *)
+    (*       (* k=k' *) *)
+    (*       apply IS.add_1. *)
+    (*       auto. *)
+    (*     + *)
+    (*       (* k!=k' *) *)
+    (*       apply ISP.FM.add_neq_iff; try auto. *)
+    (*       apply IHl. *)
+    (*       * *)
+    (*         inversion U. *)
+    (*         auto. *)
+    (*       * *)
+    (*         eapply IP.F.add_neq_in_iff with (x:=k'). *)
+    (*         auto. *)
+    (*         apply H. *)
+    (* Qed. *)
+
+    (* Lemma IM_key_in_elements : *)
+    (*   forall k elt m, *)
+    (*     IM.In (elt:=elt) k m -> *)
+    (*     In k (map fst (IM.elements (elt:=elt) m)). *)
+    (* Proof. *)
+    (*   intros k elt m H. *)
+    (*   apply NM_NS_In in H. *)
+    (*   pose proof (IM.elements_3w m) as U. *)
+    (*   generalize dependent (IM.elements m). intros l U H. *)
+    (*   induction l. *)
+    (*   - *)
+    (*     cbn in U. *)
+    (*     apply ISP.FM.empty_iff in U. *)
+    (*     trivial. *)
+    (*   - *)
+    (*     destruct a as [k' v]. *)
+    (*     simpl in *. *)
+    (*     destruct (Z.eq_decidable k k') as [K|NK]. *)
+    (*     + *)
+    (*       (* k=k' *) *)
+    (*       left. *)
+    (*       auto. *)
+    (*     + *)
+    (*       (* k!=k' *) *)
+    (*       right. *)
+    (*       apply IHl. *)
+    (*       * *)
+    (*         apply ISP.FM.add_neq_iff in U; auto. *)
+    (*       * *)
+    (*         clear IHl. *)
+    (*         inv H. *)
+    (*         auto. *)
+    (* Qed. *)
+
+    (* Lemma allocated_next_key_diff : *)
+    (*   forall m ptr, *)
+    (*     allocated ptr m -> *)
+    (*     next_logical_key m <> fst ptr. *)
+    (* Proof. *)
+    (*   intros [[cm lm] fs] [ptr_a ptr_o] H. *)
+    (*   Transparent next_logical_key. *)
+    (*   unfold next_logical_key, next_logical_key_mem, logical_next_key. *)
+    (*   cbn. *)
+    (*   unfold allocated in H. *)
+    (*   epose proof maximumBy_Z_correct. *)
+    (*   assert (In ptr_a (map fst (IM.elements (elt:=logical_block) lm))). *)
+    (*   { apply IM_key_in_elements. *)
+    (*     apply IM.mem_2; auto. *)
+    (*   } *)
+
+    (*   eapply H0 with (def:= (-1)%Z) in H1. *)
+    (*   apply Z.leb_le in H1. *)
+
+    (*   destruct (maximumBy Z.leb (-1)%Z (map fst (IM.elements (elt:=logical_block) lm))) eqn:BLAH.              - lia. *)
+    (*   - destruct p; lia. *)
+    (*   - destruct ptr_a; try lia. *)
+    (*     assert (p0 >= p)%positive by lia. *)
+    (*     assert (p = 1 \/ 1 < p)%positive by lia. *)
+    (*     destruct H3. *)
+    (*     + subst. *)
+    (*       cbn. lia. *)
+    (*     + pose proof H3. apply Z.pos_sub_lt in H3. rewrite H3. *)
+    (*       lia. *)
+    (* Qed. *)
+
+    (* Lemma get_logical_block_frames : *)
+    (*   forall cm lm f1 f2, *)
+    (*     get_logical_block ((cm, lm), f1) = get_logical_block ((cm, lm), f2). *)
+    (* Proof. *)
+    (*   intros cm lm f1 f2. *)
+    (*   unfold get_logical_block. *)
+    (*   cbn. *)
+    (*   reflexivity. *)
+    (* Qed. *)
+
+    (* Lemma get_logical_block_add_to_frame : *)
+    (*   forall m key ptr, *)
+    (*     get_logical_block (add_to_frame m key) ptr = get_logical_block m ptr. *)
+    (* Proof. *)
+    (*   intros [[cm lm] fs] key ptr. *)
+    (*   cbn. *)
+    (*   destruct fs; *)
+    (*     erewrite get_logical_block_frames; reflexivity. *)
+    (* Qed. *)
+
+    (* Lemma get_logical_block_allocated: *)
+    (*   forall m1 m2 τ ptr ptr_allocated, *)
+    (*     allocate m1 τ = inr (m2, ptr_allocated) -> *)
+    (*     allocated ptr m1 -> *)
+    (*     get_logical_block m2 (fst ptr) = get_logical_block m1 (fst ptr). *)
+    (* Proof. *)
+    (*   Opaque add_logical_block next_logical_key. *)
+    (*   intros [[cm1 lm1] fs1] [[cm2 lm2] fs2] τ ptr ptr_allocated ALLOC INm1. *)
+    (*   pose proof (allocate_correct ALLOC) as (ALLOC_FRESH & ALLOC_NEW & ALLOC_OLD). *)
+    (*   unfold allocate in ALLOC. *)
+    (*   destruct τ; inversion ALLOC. *)
+    (*   all : *)
+    (*     rewrite get_logical_block_add_to_frame; *)
+    (*     rewrite get_logical_block_of_add_logical_block_neq; *)
+    (*     [auto | apply allocated_next_key_diff; auto]. *)
+    (*   Transparent add_logical_block next_logical_key. *)
+    (* Qed. *)
+
+    (* Lemma dtyp_fits_after_allocated: *)
+    (*   forall m1 m2 τ ptr τ' ptr_allocated, *)
+    (*     allocate m1 τ = inr (m2, ptr_allocated) -> *)
+    (*     dtyp_fits m1 ptr τ' -> *)
+    (*     dtyp_fits m2 ptr τ'. *)
+    (* Proof. *)
+    (*   intros m1 m2 τ ptr τ' ptr_allocated ALLOC FITS. *)
+    (*   pose proof FITS as ALLOCATED. *)
+    (*   apply dtyp_fits_allocated in ALLOCATED. *)
+    (*   pose proof (freshly_allocated_different_blocks _ _ _ ALLOC ALLOCATED) as DIFF. *)
+
+    (*   unfold dtyp_fits in *. *)
+    (*   erewrite get_logical_block_allocated; eauto. *)
+    (* Qed. *)
+
+    (* Lemma handle_gep_addr_allocated : *)
+    (*   forall idxs sz τ ptr m elem_addr, *)
+    (*     allocated ptr m -> *)
+    (*     handle_gep_addr (DTYPE_Array sz τ) ptr idxs = inr elem_addr -> *)
+    (*     allocated elem_addr m. *)
+    (* Proof. *)
+    (*   induction idxs; *)
+    (*     intros sz τ [b i] m [eb ei] ALLOC GEP. *)
+    (*   - discriminate GEP. *)
+    (*   - cbn in *. destruct a; inversion GEP. *)
+    (*     + destruct (handle_gep_h (DTYPE_Array sz τ) (i + Z.of_N (sz * sizeof_dtyp τ) * DynamicValues.Int32.unsigned x) idxs); inversion GEP; subst. *)
+    (*       apply ALLOC. *)
+    (*     + destruct (handle_gep_h (DTYPE_Array sz τ) (i + Z.of_N (sz * sizeof_dtyp τ) * DynamicValues.Int64.unsigned x) idxs); inversion GEP; subst. *)
+    (*       apply ALLOC. *)
+    (* Qed. *)
+
+    (* (* ext_memory only talks in terms of reads... Does not *)
+    (*    necessarily preserved what's allocated, because you might *)
+    (*    not be able to read from an allocated block *) *)
+    (* Lemma ext_memory_trans : *)
+    (*   forall m1 m2 m3 τ v1 v2 dst, *)
+    (*     ext_memory m1 dst τ v1 m2 -> *)
+    (*     ext_memory m2 dst τ v2 m3 -> *)
+    (*     ext_memory m1 dst τ v2 m3. *)
+    (* Proof. *)
+    (*   intros m1 m2 m3 τ v1 v2 dst [NEW1 OLD1] [NEW2 OLD2]. *)
+    (*   split; auto. *)
+    (*   intros a' τ' ALLOC DISJOINT. *)
+    (*   rewrite <- OLD1; eauto. *)
+    (*   pose proof (allocated_can_read _ _ τ' ALLOC) as [v READ]. *)
+    (*   rewrite <- OLD1 in READ; eauto. *)
+    (*   apply can_read_allocated in READ. *)
+    (*   rewrite <- OLD2; eauto. *)
+    (* Qed. *)
+
+    (* (* If I write to a different area, it doesn't affect the allocation of other addresses *) *)
+    (* Lemma write_untouched_allocated: *)
+    (*   forall m1 m2 a τa v, *)
+    (*     dvalue_has_dtyp v τa -> *)
+    (*     write m1 a v = inr m2 -> *)
+    (*     forall b τb, no_overlap_dtyp a τa b τb -> *)
+    (*             allocated b m2 -> *)
+    (*             allocated b m1. *)
+    (* Proof. *)
+    (*   intros m1 m2 a τa v TYP WRITE b τb OVERLAP ALLOC. *)
+
+    (*   eapply allocated_can_read in ALLOC as [v' READ]. *)
+    (*   eapply can_read_allocated. *)
+
+    (*   erewrite write_untouched in READ; eauto. *)
+    (* Qed. *)
+
+    (* Lemma write_get_logical_block_neq : *)
+    (*   forall (m m' : memory_stack) (t : dtyp) (val : dvalue) (a a' : addr) (i i' : nat), *)
+    (*     write m a val = inr m' -> *)
+    (*     fst a' <> fst a -> *)
+    (*     get_logical_block m (fst a') = get_logical_block m' (fst a'). *)
+    (* Proof. *)
+    (*   intros m m' t val a a' i i' WRITE NEQ. *)
+    (*   unfold write in WRITE. *)
+    (*   break_match_hyp. *)
+    (*   - destruct l, a. *)
+    (*     cbn in WRITE; inv WRITE. *)
+    (*     symmetry. *)
+    (*     apply get_logical_block_of_add_logical_frame_ineq. *)
+    (*     eauto. *)
+    (*   - inv WRITE. *)
+    (* Qed. *)
+
+    (* Lemma write_untouched_ptr_block_get_array_cell : *)
+    (*   forall (m m' : memory_stack) (t : dtyp) (val : dvalue) (a a' : addr) (i i' : nat), *)
+    (*     write m a val = inr m' -> *)
+    (*     fst a' <> fst a -> *)
+    (*     get_array_cell m' a' i' t = get_array_cell m a' i' t. *)
+    (* Proof. *)
+    (*   intros m m' t val a a' i i' WRITE NEQ. *)
+
+    (*   destruct a as [b1 o1]. *)
+    (*   destruct a' as [b2 o2]. *)
+    (*   unfold get_array_cell. *)
+
+    (*   assert (get_logical_block m b2 = get_logical_block m' b2). *)
+    (*   { change b2 with (fst (b2, o2)). *)
+    (*     eapply write_get_logical_block_neq; eauto. *)
+    (*   } *)
+
+    (*   rewrite H. *)
+    (*   reflexivity. *)
+    (* Qed. *)
+
+    (* Lemma no_overlap_dtyp_array_different_indices: *)
+    (*   forall ix i ptrll elem_addr1 elem_addr2 sz τ, *)
+    (*     handle_gep_addr (DTYPE_Array sz τ) ptrll [DVALUE_I64 (repr 0); DVALUE_I64 ix] = inr elem_addr1 -> *)
+    (*     Int64.unsigned i <> Int64.unsigned ix -> *)
+    (*     handle_gep_addr (DTYPE_Array sz τ) ptrll [DVALUE_I64 (repr 0); DVALUE_I64 i] = inr elem_addr2 -> *)
+    (*     no_overlap_dtyp elem_addr1 τ elem_addr2 τ. *)
+    (* Proof. *)
+    (*   intros ix i [ptr_b ptr_o] elem_addr1 elem_addr2 sz τ GEP1 NEQ GEP2. *)
+    (*   unfold handle_gep_addr in *. *)
+    (*   cbn in *; inv GEP1; inv GEP2. *)
+    (*   unfold no_overlap_dtyp. red. *)
+    (*   cbn. *)
+    (*   right. *)
+
+    (*   rewrite Integers.Int64.unsigned_repr; [|cbn; lia]. *)
+
+    (*   replace (ptr_o + Z.of_N (sz * sizeof_dtyp τ) * 0 + Int64.unsigned ix * Z.of_N (sizeof_dtyp τ)) *)
+    (*     with *)
+    (*       (ptr_o + Int64.unsigned ix * Z.of_N (sizeof_dtyp τ)) by lia. *)
+    (*   replace (ptr_o + Z.of_N (sz * sizeof_dtyp τ) * 0 + Int64.unsigned i * Z.of_N (sizeof_dtyp τ) + Z.of_N (sizeof_dtyp τ) - 1) *)
+    (*     with *)
+    (*       (ptr_o + Int64.unsigned i * Z.of_N (sizeof_dtyp τ) + Z.of_N (sizeof_dtyp τ) - 1) by lia. *)
+
+    (*   pose proof (ZArith_dec.Z_lt_le_dec (DynamicValues.Int64.unsigned i) (DynamicValues.Int64.unsigned ix)) as [LT | LE]. *)
+    (*   - left. *)
+    (*     assert (Int64.unsigned i * Z.of_N (sizeof_dtyp τ) <= (Int64.unsigned ix * Z.of_N (sizeof_dtyp τ) - Z.of_N (sizeof_dtyp τ))). *)
+    (*     { replace (Int64.unsigned ix * Z.of_N (sizeof_dtyp τ) - Z.of_N (sizeof_dtyp τ)) with (Int64.unsigned ix * Z.of_N (sizeof_dtyp τ) - (1 * Z.of_N (sizeof_dtyp τ))) by lia. *)
+    (*       rewrite <- Z.mul_sub_distr_r. *)
+    (*       apply Zmult_le_compat_r; lia. *)
+    (*     } *)
+
+    (*     lia. *)
+    (*   - right. *)
+    (*     assert (Int64.unsigned ix * Z.of_N (sizeof_dtyp τ) <= (Int64.unsigned i * Z.of_N (sizeof_dtyp τ) - Z.of_N (sizeof_dtyp τ))). *)
+    (*     { replace (Int64.unsigned i * Z.of_N (sizeof_dtyp τ) - Z.of_N (sizeof_dtyp τ)) with (Int64.unsigned i * Z.of_N (sizeof_dtyp τ) - (1 * Z.of_N (sizeof_dtyp τ))) by lia. *)
+    (*       rewrite <- Z.mul_sub_distr_r. *)
+    (*       apply Zmult_le_compat_r; lia. *)
+    (*     } *)
+        
+    (*     lia. *)
+    (* Qed. *)
+
+    (* Definition equiv : memory_stack -> memory_stack -> Prop := *)
+    (*   fun '((cm,lm), s) '((cm',lm'),s') => *)
+    (*     equivs s s' /\ *)
+    (*     equivc cm cm' /\ *)
+    (*     equivl lm lm'. *)
+
+    (* #[global] Instance equiv_Equiv : Equivalence equiv. *)
+    (* Proof. *)
+    (*   split. *)
+    (*   - intros ((cm,lm),s); cbn; split; [| split]; reflexivity. *)
+    (*   - intros ((cm,lm),s) ((cm',lm'),s') EQ; cbn; split; [| split]; symmetry; apply EQ. *)
+    (*   - intros ((cm,lm),s) ((cm',lm'),s') ((cm'',lm''),s'') EQ1 EQ2; cbn; split; [| split]; (etransitivity; [apply EQ1 | apply EQ2]). *)
+    (* Qed. *)
+
+    (* Infix "≡" := equiv (at level 25). *)
+
+    (* Lemma add_add_logical : forall off b1 b2 m, *)
+    (*     equivl (add off b2 (add off b1 m)) (add off b2 m). *)
+    (* Proof. *)
+    (*   intros; apply Equiv_add_add. *)
+    (* Qed. *)
+
+    (* Lemma add_logical_block_add_logical_block : *)
+    (*   forall off b1 b2 m, *)
+    (*     add_logical_block off b2 (add_logical_block off b1 m) ≡ add_logical_block off b2 m. *)
+    (* Proof. *)
+    (*   intros ? ? ? ((cm,lm),s). *)
+    (*   cbn; split; [reflexivity | split; [reflexivity |]]. *)
+    (*   apply add_add_logical. *)
+    (* Qed. *)
+
+    (* #[global] Instance Proper_add_logical : Proper (Logic.eq ==> equivlb ==> equivl ==> equivl) add. *)
+    (* Proof. *)
+    (*   repeat intro; subst. *)
+    (*   destruct H1 as [DOM EQUIV]. *)
+    (*   split. *)
+    (*   - intros k; destruct (RelDec.rel_dec_p k y); [subst; rewrite 2 member_add_eq; auto | rewrite 2 member_add_ineq; auto]; reflexivity. *)
+    (*   - intros k; destruct (RelDec.rel_dec_p k y); [subst; rewrite 2 lookup_add_eq; auto | rewrite 2 lookup_add_ineq; auto]. *)
+    (*     intros v v' EQ1 EQ2; inv EQ1; inv EQ2; auto. *)
+    (*     intros v v' EQ1 EQ2. *)
+    (*     eapply EQUIV; eauto. *)
+    (* Qed. *)
+
+    (* #[global] Instance Proper_add_logical_block : *)
+    (*   Proper (Logic.eq ==> equivlb ==> equiv ==> equiv) add_logical_block. *)
+    (* Proof. *)
+    (*   repeat intro; subst. *)
+    (*   destruct x1 as ((mc,ml),s), y1 as ((mc',ml'),s'), H1 as (? & ? & EQ); cbn in *. *)
+    (*   split; [| split]; auto. *)
+    (*   rewrite EQ, H0. *)
+    (*   reflexivity. *)
+    (* Qed. *)
+
+    (* #[global] Instance Proper_LBlock : Proper (Logic.eq ==> Equal ==> Logic.eq ==> equivlb) LBlock. *)
+    (* Proof. *)
+    (*   repeat intro; subst. *)
+    (*   constructor; auto. *)
+    (* Qed. *)
+
+    (* (* YZ : Either exists, or define more properly *) *)
+    (* Definition equiv_sum {A : Type} (R : A -> A -> Prop) : err A -> err A -> Prop := *)
+    (*   fun ma ma' => match ma,ma' with *)
+    (*                 | inr a, inr a' => R a a' *)
+    (*                 | inl _, inl _ => True *)
+    (*                 | _, _ => False *)
+    (*                 end. *)
+
+    (* Lemma write_write : *)
+    (*   forall (m : memory_stack) (v1 v2 : dvalue) (a : addr) τ, *)
+    (*     dvalue_has_dtyp v1 τ -> *)
+    (*     dvalue_has_dtyp v2 τ -> *)
+    (*     equiv_sum equiv ('m1 <- write m a v1;; write m1 a v2) (write m a v2). *)
+    (* Proof. *)
+    (*   intros * T1 T2. *)
+    (*   unfold write; cbn. *)
+    (*   flatten_goal; repeat flatten_hyp Heq; try inv_sum. *)
+    (*   reflexivity. *)
+    (*   cbn in *. *)
+    (*   rewrite get_logical_block_of_add_logical_block. *)
+    (*   cbn. *)
+    (*   rewrite add_all_index_twice. *)
+    (*   apply add_logical_block_add_logical_block. *)
+    (*   erewrite 2 Zlength_correct. *)
+    (*   do 2 rewrite <- nat_N_Z. *)
+    (*   erewrite 2 sizeof_serialized; eauto. *)
+    (* Qed. *)
+
+    (* Lemma write_different_blocks : *)
+    (*   forall m m2 p p' v v2 dv2 τ τ', *)
+    (*     write m p v = inr m2 -> *)
+    (*     read m p' τ = inr v2 -> *)
+    (*     fst p <> fst p' -> *)
+    (*     uvalue_to_dvalue v2 = inr dv2 -> *)
+    (*     dvalue_has_dtyp dv2 τ -> *)
+    (*     dvalue_has_dtyp v τ' -> *)
+    (*     read m2 p' τ = inr v2. *)
+    (* Proof. *)
+    (*   intros m m2 p p' v v2 dv2 τ τ' WRITE READ NEQ UVDV TYP1 TYP2. *)
+    (*   erewrite write_untouched; eauto. *)
+    (*   unfold no_overlap_dtyp. *)
+    (*   unfold no_overlap. *)
+    (*   left. auto. *)
+    (* Qed. *)
+
+    (* Lemma read_in_mem_block_type : *)
+    (*   forall bytes a τ v, *)
+    (*     is_supported τ -> *)
+    (*     read_in_mem_block bytes a τ = v -> *)
+    (*     uvalue_has_dtyp v τ. *)
+    (* Proof. *)
+    (*   intros bytes a τ v SUP READ. *)
+
+    (*   unfold read_in_mem_block in READ. *)
+    (*   unfold deserialize_sbytes in READ. *)
+    (*   break_match_hyp. *)
+    (*   2: { *)
+    (*     (* If any byte is undef, then we get a UVALUE_Undef of the appropriate type *) *)
+    (*     subst. *)
+    (*     constructor. *)
+    (*   } *)
+
+    (*   (* Issue with pointers deserializing to None... *) *)
+    (* Admitted. *)
+
+    (* Lemma read_type : *)
+    (*   forall m p τ v, *)
+    (*     is_supported τ -> *)
+    (*     read m p τ = inr v -> *)
+    (*     uvalue_has_dtyp v τ. *)
+    (* Proof. *)
+    (*   intros m p τ v SUP READ. *)
+    (*   unfold read in *. *)
+    (*   break_match; inversion READ. *)
+    (*   clear H0. *)
+    (*   break_match; subst. *)
+    (*   inversion READ. *)
+    (*   eapply read_in_mem_block_type; eauto. *)
+    (* Qed. *)
+
+End Memory_Stack_Theory.
+
+Section PARAMS.
+  Variable (E F G : Type -> Type).
+  Context `{FailureE -< F} `{UBE -< F} `{PickE -< F}.
+  Notation Effin := (E +' IntrinsicE +' MemoryE +' F).
+  Notation Effout := (E +' F).
+  Notation interp_memory := (@interp_memory E F _ _ _).
+
+  Section Structural_Lemmas.
+
+    Lemma interp_memory_bind :
+      forall (R S : Type) (t : itree Effin R) (k : R -> itree Effin S) ms,
+        interp_memory (ITree.bind t k) ms ≅
+                      ITree.bind (interp_memory t ms) (fun '(ms', r) => interp_memory (k r) ms').
+    Proof.
+      intros.
+      unfold interp_memory.
+      setoid_rewrite interp_state_bind.
+      apply eq_itree_clo_bind with (UU := Logic.eq).
+      reflexivity.
+      intros [] [] EQ; inv EQ; reflexivity.
+    Qed.
+
+    Lemma interp_memory_ret :
+      forall (R : Type) m (x: R),
+        interp_memory (Ret x: itree Effin R) m ≅ Ret (m,x).
+    Proof.
+      intros; apply interp_state_ret.
+    Qed.
+
+    Lemma interp_memory_Tau :
+      forall {R} (t: itree Effin R) m,
+        interp_memory (Tau t) m ≅ Tau (interp_memory t m).
+    Proof.
+      intros.
+      unfold interp_memory; rewrite interp_state_tau; reflexivity.
+    Qed.
+
+    Lemma interp_memory_vis_eqit:
+      forall S X (kk : X -> itree Effin S) m
+             (e : Effin X),
+        interp_memory (Vis e kk) m ≅ ITree.bind (interp_memory_h e m) (fun sx => Tau (interp_memory (kk (snd sx)) (fst sx))).
+    Proof.
+      intros.
+      unfold interp_memory.
+      setoid_rewrite interp_state_vis.
+      reflexivity.
+    Qed.
+
+    Lemma interp_memory_vis:
+      forall m S X (kk : X -> itree Effin S) (e : Effin X),
+        interp_memory (Vis e kk) m ≈ ITree.bind (interp_memory_h e m) (fun sx => interp_memory (kk (snd sx)) (fst sx)).
+    Proof.
+      intros.
+      rewrite interp_memory_vis_eqit.
+      apply eutt_eq_bind.
+      intros ?; tau_steps; reflexivity.
+    Qed.
+
+    Lemma interp_memory_trigger:
+      forall (m : MemState) X (e : Effin X),
+        interp_memory (ITree.trigger e) m ≈ interp_memory_h e m.
+    Proof.
+      intros.
+      unfold interp_memory.
+      rewrite interp_state_trigger.
+      reflexivity.
+    Qed.
+
+    Lemma interp_memory_bind_trigger_eqit:
+      forall m S X (kk : X -> itree Effin S) (e : Effin X),
+        interp_memory (ITree.bind (trigger e) kk) m ≅ ITree.bind (interp_memory_h e m) (fun sx => Tau (interp_memory (kk (snd sx)) (fst sx))).
+    Proof.
+      intros.
+      unfold interp_memory.
+      rewrite bind_trigger.
+      setoid_rewrite interp_state_vis.
+      reflexivity.
+    Qed.
+
+    Lemma interp_memory_bind_trigger:
+      forall m S X
+             (kk : X -> itree Effin S)
+             (e : Effin X),
+        interp_memory (ITree.bind (trigger e) kk) m ≈ ITree.bind (interp_memory_h e m) (fun sx => interp_memory (kk (snd sx)) (fst sx)).
+    Proof.
+      intros.
+      rewrite interp_memory_bind_trigger_eqit.
+      apply eutt_eq_bind.
+      intros ?; tau_steps; reflexivity.
+    Qed.
+
+    #[global] Instance eutt_interp_memory {R} :
+      Proper (eutt Logic.eq ==> Logic.eq ==> eutt Logic.eq) (@interp_memory R).
+    Proof.
+      repeat intro.
+      unfold interp_memory.
+      subst; rewrite H2.
+      reflexivity.
+    Qed.
+
+    Lemma interp_memory_load :
+      forall (m : MemState) (t : dtyp) (val : uvalue) (a : addr),
+        read (ms_memory_stack m) a t = inr val ->
+        interp_memory (trigger (Load t (DVALUE_Addr a))) m ≈ Ret (m, val).
+    Proof.
+      intros [ms sid pr] t val a Hval.
+      rewrite interp_memory_trigger.
+      cbn in Hval.
+      cbn.
+      rewrite bind_ret_l.
+      rewrite bind_ret_l.
+      cbn.
+      rewrite Hval.
+      reflexivity.
+    Qed.
+
+    Lemma interp_memory_store :
+      forall (m m' : MemState) (val : uvalue) (dt : dtyp) (a : addr),
+        ErrSID_MemState_ms_runs_to (fun ms => write ms a val dt) m m' ->
+        interp_memory (trigger (Store dt (DVALUE_Addr a) val)) m ≈ Ret (m', tt).
+    Proof.
+      intros m m' val dt a Hwrite.
+      rewrite interp_memory_trigger.
+      cbn.
+      repeat rewrite bind_ret_l.
+      cbn.
+      rewrite Hwrite.
+      repeat rewrite bind_ret_l; cbn.
+      destruct m, m'; cbn.
+      reflexivity.
+    Qed.
+
+    Lemma interp_memory_store_exists :
+      forall (m : MemState) (t : dtyp) (val : uvalue) (a : addr) aids,
+        uvalue_has_dtyp val t ->
+        write_allowed (fst (ms_memory_stack m)) (fst a) (snd a) (N.to_nat (sizeof_dtyp t)) = inr aids ->
+        exists m',
+          ErrSID_MemState_ms_runs_to (fun ms => write ms a val t) m m' /\
+          interp_memory (trigger (Store t (DVALUE_Addr a) val)) m ≈ Ret (m', tt).
+    Proof.
+      intros m t val a aids TYP CAN.
+      apply write_succeeds with (v:=val) in CAN as [m2 WRITE]; auto.
+      exists m2. split; auto.
+
+      eapply interp_memory_store; eauto.
+    Qed.
+
+    Lemma interp_memory_alloca :
+      forall (m m' : MemState) (t : dtyp) (a : addr),
+        ErrSID_runs_to (allocate (ms_memory_stack m) t) (ms_sid m) (ms_prov m) (ms_memory_stack m', a) (ms_sid m') (ms_prov m') ->
+        interp_memory (trigger (Alloca t)) m ≈ Ret (m', DVALUE_Addr a).
+    Proof.
+      intros m m' t a ALLOC.
+      rewrite interp_memory_trigger.
+      cbn in *.
+      repeat rewrite bind_ret_l; cbn.
+      rewrite ALLOC. 
+      repeat rewrite bind_ret_l; cbn.
+      repeat rewrite bind_ret_l; cbn.
+      destruct m, m'; cbn.
+      reflexivity.
+    Qed.
+
+ (*    Lemma interp_memory_alloca_exists : *)
+ (*      forall (m : memory_stack) (t : dtyp), *)
+ (*        non_void t -> *)
+ (*        exists m' a', allocate m t = inr (m', a') /\ *)
+ (*                      interp_memory (trigger (Alloca t)) m ≈ Ret (m', DVALUE_Addr a'). *)
+ (*    Proof. *)
+ (*      intros m t NV. *)
+ (*      apply allocate_succeeds with (τ:=t) (m1:=m) in NV as [m' [a' ALLOC]]. *)
+ (*      exists m'. exists a'. *)
+ (*      auto using interp_memory_alloca. *)
+ (*    Qed. *)
+
+ (*    Lemma lookup_all_add_all_app : *)
+ (*      forall (xs ys : list SByte) o bytes def, *)
+ (*        lookup_all_index o (N.of_nat (List.length xs + List.length ys)) (add_all_index (xs ++ ys) o bytes) def = xs ++ lookup_all_index (o + Z.of_nat (List.length xs)) (N.of_nat (List.length ys)) (add_all_index (xs ++ ys) o bytes) def. *)
+ (*    Proof. *)
+ (*    Abort. *)
+
+ (*    Lemma lookup_all_add_all : *)
+ (*      forall o bytes (sbytes : list SByte) def, *)
+ (*        lookup_all_index o (N.of_nat (List.length sbytes)) (add_all_index sbytes o bytes) def = sbytes. *)
+ (*    Proof. *)
+ (*      intros o bytes sbytes def. *)
+ (*      induction sbytes. *)
+ (*      - reflexivity. *)
+ (*      - cbn in *. *)
+ (*    Abort. *)
+
+ (*    Lemma get_array_succeeds_allocated : forall m a i t val, *)
+ (*        get_array_cell m a i t = inr val -> *)
+ (*        allocated a m. *)
+ (*    Proof. *)
+ (*      intros m [b o] i t val GET. *)
+ (*      cbn in GET. *)
+ (*      unfold get_logical_block in GET. *)
+ (*      unfold get_logical_block_mem in GET. *)
+ (*      break_match; inv GET. *)
+
+ (*      apply lookup_member in Heqo0. *)
+ (*      destruct m as [[lm cm] f]. *)
+ (*      cbn in *. auto. *)
+ (*    Qed. *)
+
+ (*    Lemma interp_memory_GEP_array_addr : forall t a (size :N) m val i ptr, *)
+ (*        get_array_cell m a i t = inr val -> *)
+ (*          handle_gep_addr (DTYPE_Array size t) a [DVALUE_I64 (Int64.repr 0); DVALUE_I64 (Int64.repr (Z.of_nat i))] = inr ptr -> *)
+ (*          interp_memory (trigger (GEP *)
+ (*                                    (DTYPE_Array size t) *)
+ (*                                    (DVALUE_Addr a) *)
+ (*                                    [DVALUE_I64 (repr 0); DVALUE_I64 (repr (Z.of_nat i))])) m *)
+ (*                        ≈ Ret (m, DVALUE_Addr ptr) /\ *)
+ (*          read m ptr t = inr val. *)
+ (*    Proof. *)
+ (*      intros * GET. intros. *)
+ (*      pose proof get_array_succeeds_allocated _ _ _ _ GET as ALLOC. *)
+ (*      pose proof @read_array m size t i a ptr ALLOC as RARRAY. *)
+ (*      split. *)
+ (*      - rewrite interp_memory_trigger. cbn. *)
+ (*        cbn in RARRAY. destruct RARRAY. auto. *)
+ (*        rewrite H2. cbn. *)
+ (*        rewrite bind_ret_l. cbn. reflexivity. *)
+ (*      - destruct RARRAY. eauto. *)
+ (*        auto. *)
+ (*    Qed. *)
+
+ (*    Lemma interp_memory_GEP_array' : forall t a size m val i, *)
+ (*        get_array_cell m a i t = inr val -> *)
+ (*        exists ptr, *)
+ (*          interp_memory (trigger (GEP *)
+ (*                                    (DTYPE_Array size t) *)
+ (*                                    (DVALUE_Addr a) *)
+ (*                                    [DVALUE_I64 (Int64.repr 0); DVALUE_I64 (Int64.repr (Z.of_nat i))])) m *)
+ (*                        ≈ Ret (m, DVALUE_Addr ptr) /\ *)
+ (*          handle_gep_addr (DTYPE_Array size t) a [DVALUE_I64 (repr 0); DVALUE_I64 (repr (Z.of_nat i))] = inr ptr /\ *)
+ (*          read m ptr t = inr val. *)
+ (*    Proof. *)
+ (*      intros t a size m val i GET. *)
+ (*      pose proof get_array_succeeds_allocated _ _ _ _ GET as ALLOC. *)
+ (*      pose proof read_array_exists m size t i a ALLOC as RARRAY. *)
+ (*      destruct RARRAY as (ptr & GEP & READ). *)
+ (*      exists ptr. *)
+ (*      split. *)
+ (*      - rewrite interp_memory_trigger. cbn. *)
+ (*        cbn in GEP. *)
+ (*        rewrite GEP. *)
+ (*        cbn. *)
+ (*        rewrite bind_ret_l. *)
+ (*        reflexivity. *)
+ (*      - rewrite <- GET. auto. *)
+ (*    Qed. *)
+
+ (*    Lemma interp_memory_GEP_array : forall t a size m val i, *)
+ (*        get_array_cell m a i t = inr val -> *)
+ (*        exists ptr, *)
+ (*          interp_memory (trigger (GEP *)
+ (*                                    (DTYPE_Array size t) *)
+ (*                                    (DVALUE_Addr a) *)
+ (*                                    [DVALUE_I64 (Int64.repr 0); DVALUE_I64 (Int64.repr (Z.of_nat i))])) m *)
+ (*                        ≈ Ret (m,DVALUE_Addr ptr) /\ *)
+ (*          read m ptr t = inr val. *)
+ (*    Proof. *)
+ (*      intros t a size m val i GET. *)
+ (*      epose proof (@interp_memory_GEP_array' t a size m val i GET) as [ptr GEP]. *)
+ (*      exists ptr. intuition. *)
+ (*    Qed. *)
+
+ (*    Lemma interp_memory_GEP_array_no_read_addr : forall t a size m i ptr, *)
+ (*      dtyp_fits m a (DTYPE_Array size t) -> *)
+ (*        handle_gep_addr (DTYPE_Array size t) a [DVALUE_I64 (Int64.repr 0); DVALUE_I64 (Int64.repr (Z.of_nat i))] = inr ptr -> *)
+ (*        interp_memory (trigger (GEP *)
+ (*                                  (DTYPE_Array size t) *)
+ (*                                  (DVALUE_Addr a) *)
+ (*                                  [DVALUE_I64 (Int64.repr 0); DVALUE_I64 (Int64.repr (Z.of_nat i))])) m *)
+ (*                      ≈ Ret (m, DVALUE_Addr ptr). *)
+ (*    Proof. *)
+ (*      intros * FITS HGEP. *)
+ (*      pose proof (dtyp_fits_allocated FITS) as ALLOC. *)
+ (*      pose proof @read_array m size t i a ptr ALLOC as RARRAY. *)
+ (*      destruct RARRAY. eauto. *)
+ (*      rewrite interp_memory_trigger. cbn. *)
+ (*      rewrite HGEP. cbn. *)
+ (*      rewrite bind_ret_l. *)
+ (*      reflexivity. *)
+ (*    Qed. *)
+
+ (*    Lemma interp_memory_GEP_array_no_read : forall t a size m i, *)
+ (*        dtyp_fits m a (DTYPE_Array size t) -> *)
+ (*        exists ptr, *)
+ (*          interp_memory (trigger (GEP *)
+ (*                                    (DTYPE_Array size t) *)
+ (*                                    (DVALUE_Addr a) *)
+ (*                                    [DVALUE_I64 (Int64.repr 0); DVALUE_I64 (Int64.repr (Z.of_nat i))])) m *)
+ (*                        ≈ Ret (m, DVALUE_Addr ptr) /\ *)
+ (*          handle_gep_addr (DTYPE_Array size t) a [DVALUE_I64 (repr 0); DVALUE_I64 (repr (Z.of_nat i))] = inr ptr. *)
+ (*    Proof. *)
+ (*      intros t a size m i FITS. *)
+ (*      pose proof (dtyp_fits_allocated FITS) as ALLOC. *)
+ (*      pose proof read_array_exists m size t i a ALLOC as RARRAY. *)
+ (*      destruct RARRAY as (ptr & GEP & READ). *)
+ (*      exists ptr. *)
+ (*      split. *)
+ (*      - rewrite interp_memory_trigger. cbn. *)
+ (*        cbn in GEP. *)
+ (*        rewrite GEP. *)
+ (*        cbn. *)
+ (*        rewrite bind_ret_l. *)
+ (*        reflexivity. *)
+ (*      - auto. *)
+ (*    Qed. *)
+
+ (*    Lemma no_overlap_reflect : *)
+ (*      forall x y s, reflect (no_overlap x s y s) (no_overlap_b x s y s). *)
+ (*    Proof. *)
+ (*      intros. *)
+ (*      destruct x as (x1 & x2). *)
+ (*      destruct y as (y1 & y2). *)
+ (*      match goal with *)
+ (*      | |- reflect ?L ?R => remember L as LHS; remember R as RHS *)
+ (*      end. *)
+ (*      destruct RHS; subst; constructor. *)
+ (*      - unfold no_overlap. *)
+ (*        unfold no_overlap_b in HeqRHS. *)
+ (*        cbn in *. *)
+ (*        destruct (x2 >? (y2 + s) - 1) eqn: EQ2. *)
+ (*        + rewrite Z.gtb_lt in EQ2. right. left. *)
+ (*          rewrite Z.gt_lt_iff. auto. *)
+ (*        + destruct (y2 >? (x2 + s) - 1) eqn: EQ3. *)
+ (*          * rewrite Z.gtb_lt in EQ3. right. right. *)
+ (*            rewrite Z.gt_lt_iff. auto. *)
+ (*          * destruct (x1 /~=? y1) eqn: EQ1. *)
+ (*            -- left. auto. *)
+ (*            -- cbn in HeqRHS. inversion HeqRHS. *)
+ (*      - unfold no_overlap. *)
+ (*        unfold no_overlap_b in HeqRHS. *)
+ (*        cbn in *. *)
+ (*        destruct (x1 /~=? y1) eqn: EQ1; try inversion HeqRHS. *)
+ (*        destruct (x2 >? (y2 + s) - 1) eqn: EQ2; try inversion HeqRHS. *)
+ (*        destruct (y2 >? (x2 + s) - 1) eqn: EQ3; try inversion HeqRHS. *)
+ (*        intuition; *)
+ (*          try first [rewrite Z.gt_lt_iff,<- Z.gtb_lt in H2; *)
+ (*                     rewrite H2 in EQ2; inversion EQ2 | *)
+ (*                     rewrite Z.gt_lt_iff,<- Z.gtb_lt in H2; *)
+ (*                     rewrite H2 in EQ3; inversion EQ3]. *)
+ (*        (* TODO: Write symmetric variants of Z.gtb_lt lemmas. *) *)
+ (*    Qed. *)
+
+ (*    Lemma app_prefix_eq : *)
+ (*      forall (A : Type) (a b c: list A), *)
+ (*        a = b -> a ++ c = b ++ c. *)
+ (*    Proof. *)
+ (*      intros. *)
+ (*      rewrite H2. reflexivity. *)
+ (*    Qed. *)
+
+ (*    Lemma Zseq_app : forall (off : Z) (n : N), *)
+ (*        Zseq off (N.to_nat (N.succ n)) = *)
+ (*        Zseq off (N.to_nat n) ++ [off + Z.of_N n]. *)
+ (*    Proof. *)
+ (*      intros. *)
+ (*      rewrite <- N.add_1_r. *)
+ (*      setoid_rewrite Nnat.N2Nat.inj_add; auto. *)
+ (*      unfold N.to_nat at 2. unfold Pos.to_nat. cbn. *)
+ (*      remember (N.to_nat n) as sz. *)
+ (*      assert (off_H: off + Z.of_N n = off + (Z.of_nat sz)). { *)
+ (*        rewrite Heqsz. rewrite N_nat_Z. reflexivity. *)
+ (*      } *)
+ (*      rewrite off_H. *)
+ (*      clear Heqsz off_H. *)
+ (*      revert off. *)
+ (*      induction sz. *)
+ (*      - intros. cbn. *)
+ (*        rewrite Zred_factor6 at 1. *)
+ (*        reflexivity. *)
+ (*      - intros. *)
+ (*        rewrite Nat.add_1_r in *. *)
+ (*        cbn in *. *)
+ (*        specialize (IHsz (Z.succ off)). *)
+ (*        rewrite IHsz. *)
+ (*        assert (Z.succ off + Z.of_nat sz = off + Z.pos (Pos.of_succ_nat sz)) as END by lia. *)
+ (*        rewrite END. reflexivity. *)
+ (*    Qed. *)
+
+ (*    Lemma Zseq_app_Z : forall off n : Z, *)
+ (*        0 <= n -> *)
+ (*        Zseq off (Z.to_nat (Z.succ n)) = *)
+ (*        Zseq off (Z.to_nat n) ++ [off + n]. *)
+ (*    Proof. *)
+ (*      intros. *)
+ (*      unfold Z.succ. *)
+ (*      setoid_rewrite Z2Nat.inj_add; auto. *)
+ (*      unfold Z.to_nat at 2. unfold Pos.to_nat. cbn. *)
+ (*      remember (Z.to_nat n) as sz. *)
+ (*      assert (off_H: off + n = off + (Z.of_nat sz)). { *)
+ (*        rewrite Heqsz. rewrite Z2Nat.id. reflexivity. auto. *)
+ (*      } *)
+ (*      rewrite off_H. *)
+ (*      clear Heqsz off_H. *)
+ (*      revert off. *)
+ (*      induction sz. *)
+ (*      - intros. cbn. *)
+ (*        setoid_rewrite Zred_factor6 at 1. *)
+ (*        reflexivity. *)
+ (*      - intros. *)
+ (*        rewrite Nat.add_1_r in *. *)
+ (*        cbn in *. *)
+ (*        specialize (IHsz (Z.succ off)). *)
+ (*        rewrite IHsz. *)
+ (*        assert (Z.succ off + Z.of_nat sz = off + Z.pos (Pos.of_succ_nat sz)) by lia. *)
+ (*        rewrite H3. reflexivity. *)
+ (*      - lia. *)
+ (*    Qed. *)
+
+ (*    Lemma list_nth_z_length: *)
+ (*      forall A (l : list A) (a : A), *)
+ (*        list_nth_z (l ++ [a]) (Z.of_nat (length l)) = Some a. *)
+ (*    Proof. *)
+ (*      intros. revert a. *)
+ (*      remember (Datatypes.length l) as LEN. revert LEN HeqLEN. *)
+ (*      induction l. *)
+ (*      - intros; subst; auto. *)
+ (*      - intros; cbn. *)
+ (*        assert ((Datatypes.length (a :: l) <> 0)%nat). *)
+ (*        { cbn. lia. } *)
+ (*        rewrite <- HeqLEN in H2. *)
+ (*        destruct (zeq (Z.of_nat LEN) 0) eqn: LENZERO. *)
+ (*        + intuition. (* absurd case *) *)
+ (*        + rewrite <- Nat2Z.inj_pred. 2 : lia. *)
+ (*          apply IHl. cbn in HeqLEN. lia. *)
+ (*    Qed. *)
+
+ (*    Lemma list_singleton_eq: *)
+ (*      forall A (a b: A), a = b -> [a] = [b]. *)
+ (*    Proof. *)
+ (*      intros. rewrite H2. reflexivity. *)
+ (*    Qed. *)
+
+ (*    Lemma lookup_all_index_add_all_length_app: *)
+ (*      forall a sz l l' offset bytes (def : a), *)
+ (*        length l = sz -> *)
+ (*        lookup_all_index offset (N.of_nat sz) *)
+ (*                         (add_all_index (l ++ l') offset bytes) def = *)
+ (*        lookup_all_index offset (N.of_nat sz) *)
+ (*                         (add_all_index l offset bytes) def. *)
+ (*    Proof. *)
+ (*      intros*. revert def bytes offset sz. *)
+ (*      induction l. *)
+ (*      - intros; cbn. cbn in H2. subst. auto. *)
+ (*      - intros; cbn in *. subst. *)
+ (*        rewrite Nnat.Nat2N.inj_succ. *)
+ (*        rewrite 2 lookup_all_index_add. *)
+ (*        rewrite IHl. reflexivity. reflexivity. *)
+ (*    Qed. *)
+
+
+ (*    (* TODO: move *) *)
+ (*    Lemma Zlength_map: *)
+ (*      forall {A B} (f : A -> B) (l : list A), *)
+ (*        Zlength (map f l) = Zlength l. *)
+ (*    Proof. *)
+ (*      intros A B f l. *)
+ (*      induction l. *)
+ (*      - reflexivity. *)
+ (*      - rewrite map_cons. *)
+ (*        rewrite 2 Zlength_cons. *)
+ (*        rewrite IHl. *)
+ (*        reflexivity. *)
+ (*    Qed. *)
+
+ (*    (* TODO: move *) *)
+ (*    Lemma Zlength_app: *)
+ (*      forall {A} (l1 l2 : list A), *)
+ (*        Zlength (l1 ++ l2) = Zlength l1 + Zlength l2. *)
+ (*    Proof. *)
+ (*      intros A; induction l1; intros l2. *)
+ (*      - reflexivity. *)
+ (*      - (* TODO: avoid this... *) *)
+ (*        Opaque Zlength. *)
+ (*        cbn. *)
+ (*        rewrite 2 Zlength_cons. *)
+ (*        Transparent Zlength. *)
+ (*        rewrite Z.add_succ_l. *)
+ (*        rewrite IHl1. *)
+ (*        reflexivity. *)
+ (*    Qed. *)
+
+ (*    Lemma Zlength_Zseq: *)
+ (*      forall sz start, *)
+ (*        Zlength (Zseq start sz) = Z.of_nat sz. *)
+ (*    Proof. *)
+ (*      induction sz; intros start. *)
+ (*      - reflexivity. *)
+ (*      - (* TODO: avoid this... *) *)
+ (*        Opaque Zlength. *)
+ (*        cbn. *)
+ (*        rewrite Zlength_cons. *)
+ (*        Transparent Zlength. *)
+ (*        rewrite IHsz. *)
+ (*        lia. *)
+ (*    Qed. *)
+
+ (*    Lemma lookup_all_index_add_all_index : *)
+ (*      forall (sz : nat) src_bytes src_offset dst_bytes dst_offset def, *)
+ (*        (lookup_all_index dst_offset (N.of_nat sz) *)
+ (*                          (add_all_index *)
+ (*                             (lookup_all_index src_offset (N.of_nat sz) src_bytes def) *)
+ (*                             dst_offset dst_bytes) SUndef) = *)
+ (*        (lookup_all_index src_offset (N.of_nat sz) src_bytes def). *)
+ (*    Proof. *)
+ (*      intros sz src_bytes src_offset dst_bytes dst_offset def. *)
+ (*      induction sz. *)
+ (*      - cbn; reflexivity. *)
+ (*      - assert (N.of_nat (S sz) = N.succ (N.of_nat sz)). cbn. *)
+ (*        lia. *)
+ (*        rewrite H2. *)
+ (*        unfold lookup_all_index in *. *)
+ (*        remember (fun x0 : IM.key => *)
+ (*                    match lookup x0 src_bytes with *)
+ (*                    | Some val => val *)
+ (*                    | None => def *)
+ (*                    end). *)
+ (*        rewrite 2 Zseq_app. *)
+ (*        unfold lookup_all_index in IHsz. *)
+ (*        + assert (match *)
+ (*                     lookup (dst_offset + Z.of_nat sz) *)
+ (*                            (add_all_index *)
+ (*                               (map s (Zseq src_offset (N.to_nat (N.of_nat sz)) ++ *)
+ (*                                            [src_offset + Z.of_nat sz])) *)
+ (*                               dst_offset dst_bytes) *)
+ (*                   with *)
+ (*                   | Some val => val *)
+ (*                   | None => SUndef *)
+ (*                   end = s (src_offset + Z.of_nat sz)). { *)
+ (*            erewrite lookup_add_all_index_in. Unshelve. *)
+ (*            3 : { *)
+ (*              rewrite Z.add_simpl_l. rewrite list_nth_z_map. *)
+ (*              unfold option_map. *)
+ (*              rewrite <- (@Zseq_length sz src_offset) at 3. *)
+ (*              rewrite Nnat.Nat2N.id. *)
+ (*              rewrite list_nth_z_length. reflexivity. *)
+ (*            } *)
+ (*            reflexivity. *)
+ (*            - split. *)
+ (*              + rewrite <- Z.add_0_r at 1. *)
+ (*                rewrite <- Z.add_le_mono_l. *)
+ (*                apply Zle_0_nat. *)
+ (*              + rewrite <- Z.add_sub_assoc. *)
+ (*                rewrite <- Z.add_le_mono_l. *)
+ (*                rewrite Zlength_correct. *)
+ (*                rewrite map_length. *)
+ (*                rewrite app_length. cbn. *)
+ (*                rewrite Nnat.Nat2N.id. *)
+ (*                rewrite <- Zseq_length at 1. *)
+ (*                rewrite Nat2Z.inj_add. cbn. *)
+ (*                rewrite Z.add_simpl_r. *)
+ (*                apply Z.le_refl. *)
+ (*          } *)
+ (*          rewrite 2 map_app. cbn. rewrite map_app in H3. *)
+ (*          cbn in H3. *)
+ (*          apply list_singleton_eq in H3. *)
+ (*          rewrite nat_N_Z. *)
+ (*          rewrite H3. clear H3. *)
+ (*          eapply app_prefix_eq. *)
+ (*          remember (add_all_index *)
+ (*                      (map s (Zseq src_offset (N.to_nat (N.of_nat sz))) ++ *)
+ (*                           [s (src_offset + Z.of_nat sz)]) dst_offset dst_bytes) as m. *)
+ (*          remember (add_all_index *)
+ (*                      (map s (Zseq src_offset (N.to_nat (N.of_nat sz)))) *)
+ (*                      dst_offset dst_bytes) as m'. *)
+ (*          setoid_rewrite <- IHsz at 2. *)
+ (*          match goal with *)
+ (*          | |- ?L = ?R => remember L as LHS; remember R as RHS *)
+ (*          end. *)
+ (*          assert (LHS = lookup_all_index dst_offset (N.of_nat sz) m SUndef). *)
+ (*          { *)
+ (*            rewrite HeqLHS. unfold lookup_all_index. subst. *)
+ (*            reflexivity. *)
+ (*          } *)
+ (*          assert (RHS = lookup_all_index dst_offset (N.of_nat sz) m' SUndef). *)
+ (*          { *)
+ (*            rewrite HeqRHS. unfold lookup_all_index. reflexivity. *)
+ (*          } *)
+ (*          rewrite H3, H4. *)
+ (*          rewrite Heqm, Heqm'. *)
+ (*          apply lookup_all_index_add_all_length_app. *)
+ (*          pose proof Zseq_length as Zseq_length_H. *)
+ (*          specialize (Zseq_length_H sz src_offset). *)
+ (*          rewrite Nnat.Nat2N.id. *)
+ (*          symmetry. *)
+ (*          rewrite map_length. auto. *)
+ (*    Qed. *)
+
+ (*    (* Note : For the current version of subevents, [interp_memory] must *)
+ (*        have subevent clauses assumed in Context, or else the *)
+ (*        [handle_intrinsic] handler will not get properly invoked. *) *)
+ (*    (* IY: This is specialized to DTYPE_Array for practical *)
+ (*         purposes. We could conjure a more complete definition later. *) *)
+ (*    Lemma interp_memory_intrinsic_memcpy : *)
+ (*      forall (m : memory_stack) (dst src : Addr.addr) (sz : N) *)
+ (*        (dst_val src_val : uvalue) (dτ : dtyp) volatile align, *)
+ (*        0 <= Z.of_N (sz * sizeof_dtyp dτ) <= Int32.max_unsigned -> *)
+ (*        read m dst (DTYPE_Array sz dτ) = inr dst_val -> *)
+ (*        read m src (DTYPE_Array sz dτ) = inr src_val -> *)
+ (*        no_overlap dst (Int32.unsigned (Int32.repr (Z.of_N (sz * sizeof_dtyp dτ)))) src *)
+ (*                   (Int32.unsigned (Int32.repr (Z.of_N (sz * sizeof_dtyp dτ)))) -> *)
+ (*        exists m' s, *)
+ (*          (interp_memory (trigger (Intrinsic DTYPE_Void *)
+ (*                                             "llvm.memcpy.p0i8.p0i8.i32" *)
+ (*                                             [DVALUE_Addr dst; DVALUE_Addr src; *)
+ (*                                             DVALUE_I32 (Int32.repr (Z.of_N (sizeof_dtyp (DTYPE_Array sz dτ)))); *)
+ (*                                             DVALUE_I32 align ; *)
+ (*                                             DVALUE_I1 volatile])) m ≈ *)
+ (*                         ret (m', s, DVALUE_None)) /\ *)
+ (*          read (m', s) dst (DTYPE_Array sz dτ) = inr src_val. *)
+ (*    Proof. *)
+ (*      intros m dst src i dst_val src_val dτ volatile align. *)
+ (*      intros size_H  MEM_dst MEM_src NO_OVERLAP. *)
+ (*      unfold read in MEM_dst, MEM_src. *)
+ (*      destruct (get_logical_block m (fst dst)) eqn: HM_dst. cbn in MEM_dst. *)
+ (*      destruct l. 2 : { inversion MEM_dst. } *)
+ (*      destruct (get_logical_block m (fst src)) eqn: HM_src. cbn in MEM_src. *)
+ (*      destruct l. 2 : { inversion MEM_src. } *)
+ (*      setoid_rewrite interp_memory_trigger. *)
+ (*      unfold interp_memory_h. cbn. *)
+ (*      unfold resum, ReSum_id, id_, Id_IFun. *)
+ (*      unfold handle_intrinsic. cbn. *)
+ (*      destruct m. *)
+ (*      destruct dst as (dst_base & dst_offset). *)
+ (*      destruct src as (src_base & src_offset). *)
+ (*      epose proof no_overlap_reflect as reflect_H. *)
+ (*      eapply reflect_iff in reflect_H. *)
+ (*      rewrite reflect_iff in NO_OVERLAP. clear reflect_H. *)
+ (*      setoid_rewrite NO_OVERLAP. cbn in *. *)
+ (*      setoid_rewrite HM_src. cbn. setoid_rewrite HM_dst. cbn. *)
+ (*      eexists. exists f. *)
+ (*      split; try reflexivity. *)
+ (*      rewrite <- MEM_src. unfold read. cbn. *)
+ (*      unfold read_in_mem_block. cbn. *)
+ (*      rewrite Int32.unsigned_repr. 2 : apply size_H. *)
+ (*      rewrite get_logical_block_of_add_logical_block_mem. *)
+ (*      pose proof lookup_all_index_add_all_index. *)
+ (*      specialize (H2 (N.to_nat (i * sizeof_dtyp dτ))). *)
+ (*      rewrite Nnat.N2Nat.id in H2. *)
+ (*      rewrite N2Z.id. *)
+ (*      rewrite H2. reflexivity. *)
+ (*      apply no_overlap_reflect. Unshelve. unfold addr, Addr.addr. *)
+ (*      exact (0, 0). exact (0, 0). eauto. *)
+ (*    Qed. *)
+
+  End Structural_Lemmas.
+
+ (*  (* TODO: move to appropriate place in this file *) *)
+ (*  Lemma handle_gep_addr_array_same_block : *)
+ (*    forall ptr ptr_elem ix sz τ, *)
+ (*      handle_gep_addr (DTYPE_Array sz τ) ptr *)
+ (*                      [DVALUE_I64 (repr 0); DVALUE_I64 ix] = inr ptr_elem -> *)
+ (*      fst ptr = fst ptr_elem. *)
+ (*  Proof. *)
+ (*    intros [ptrb ptro] [ptr_elemb ptr_elemo] ix sz τ GEP. *)
+ (*    cbn in GEP. *)
+ (*    inversion GEP; subst. *)
+ (*    reflexivity. *)
+ (*  Qed. *)
+
+ (*  Lemma unsigned_repr_0_i64 : *)
+ (*    DynamicValues.Int64.unsigned (DynamicValues.Int64.repr 0) = 0. *)
+ (*  Proof. *)
+ (*    apply Integers.Int64.unsigned_zero. *)
+ (*  Qed. *)
+
+
+ (*  Lemma handle_gep_addr_array_offset : *)
+ (*    forall ptr ptr_elem ix sz τ, *)
+ (*      handle_gep_addr (DTYPE_Array sz τ) ptr *)
+ (*                      [DVALUE_I64 (repr 0); DVALUE_I64 ix] = inr ptr_elem -> *)
+ (*      snd ptr + DynamicValues.Int64.unsigned ix * Z.of_N (sizeof_dtyp τ) = snd ptr_elem. *)
+ (*  Proof. *)
+ (*    intros [ptrb ptro] [ptr_elemb ptr_elemo] ix sz τ GEP. *)
+ (*    cbn in GEP. *)
+ (*    inversion GEP; subst. *)
+ (*    cbn. *)
+ (*    rewrite unsigned_repr_0_i64. *)
+ (*    lia. *)
+ (*  Qed. *)
+
+ (* Lemma dtyp_fits_array_elem : *)
+ (*    forall m ptr ptr_elem ix (sz : N) τ, *)
+ (*      dtyp_fits m ptr (DTYPE_Array sz τ) -> *)
+ (*      handle_gep_addr (DTYPE_Array sz τ) ptr *)
+ (*                      [DVALUE_I64 (repr 0); DVALUE_I64 ix] = inr ptr_elem -> *)
+ (*      Int64.intval ix < Z.of_N sz -> *)
+ (*      dtyp_fits m ptr_elem τ. *)
+ (*  Proof. *)
+ (*    intros m ptr ptr_elem ix sz τ FITS GEP SZ. *)
+ (*    cbn in GEP. *)
+ (*    unfold dtyp_fits in *. *)
+ (*    destruct FITS as (sz' & bytes & cid & BLOCK & BOUND). *)
+ (*    exists sz'. exists bytes. exists cid. *)
+ (*    split. *)
+ (*    erewrite <- handle_gep_addr_array_same_block; eauto. *)
+ (*    erewrite <- handle_gep_addr_array_offset; eauto. *)
+ (*    cbn in BOUND. *)
+ (*    assert (Int64.unsigned ix = Int64.intval ix) by reflexivity. *)
+ (*    rewrite H2. *)
+ (*    assert (1 + Int64.intval ix <= Z.of_N sz) by lia. *)
+ (*    rewrite <- Z.add_assoc. *)
+ (*    assert (snd ptr + (Int64.intval ix * Z.of_N (sizeof_dtyp τ) + Z.of_N (sizeof_dtyp τ)) <= snd ptr + Z.of_N (sz * sizeof_dtyp τ)). *)
+ (*    { eapply Zorder.Zplus_le_compat_l. *)
+ (*      replace (Int64.intval ix * Z.of_N (sizeof_dtyp τ) + Z.of_N (sizeof_dtyp τ)) with ((1 + Int64.intval ix) * Z.of_N (sizeof_dtyp τ)). *)
+ (*      rewrite N2Z.inj_mul. *)
+ (*      eapply Z.mul_le_mono_nonneg_r; lia. *)
+ (*      lia. *)
+ (*    } *)
+ (*    lia. *)
+ (*  Qed. *)
+
+End PARAMS.
+End MEMORY_THEORY.
+
+Module Make(LLVMEvents : LLVM_INTERACTIONS(Addr)) <: MEMORY_THEORY(LLVMEvents).
+Include MEMORY_THEORY(LLVMEvents).
+End Make.
